aim to the goal

coq/theories/PetitSQL.v
@@ -16,1006 +16,1647 @@ Require Import Coq.Strings.Byte.
 Require Import Coq.Strings.String.
 Require Import Coq.ZArith.BinInt.
 
+Module StringNotations.
+
+Notation char := ascii.
+
+Notation " '[' ']' " := (EmptyString) : string_scope.
+
+Notation " ch '::' str " := (String (ch)%char (str)%string) : string_scope.
+
+End StringNotations.
+
 Module Prelude.
 
-  Import ListNotations.
+Import StringNotations ListNotations.
 
-  #[universes(polymorphic=yes)]
-  Definition REFERENCE_HOLDER@{lv} {STATEMENT_Type : Type@{lv}} (REFERENCED_STATEMENT : unit -> STATEMENT_Type) : STATEMENT_Type := REFERENCED_STATEMENT tt.
+#[universes(polymorphic=yes)]
+Definition REFERENCE_HOLDER@{lv} {STATEMENT_Type : Type@{lv}} (REFERENCED_STATEMENT : unit -> STATEMENT_Type) : STATEMENT_Type := REFERENCED_STATEMENT tt.
+Notation " '<<' STATEMENT_REFERENCE ':' STATEMENT '>>' " := (REFERENCE_HOLDER (fun STATEMENT_REFERENCE : unit => match STATEMENT_REFERENCE with tt => STATEMENT end)) (STATEMENT_REFERENCE name, STATEMENT at level 200, at level 70, no associativity) : type_scope.
+Ltac unnw := unfold REFERENCE_HOLDER in *.
 
-  #[global]
-  Notation " '<<' STATEMENT_REFERENCE ':' STATEMENT '>>' " := (REFERENCE_HOLDER (fun STATEMENT_REFERENCE : unit => match STATEMENT_REFERENCE with tt => STATEMENT end)) (STATEMENT_REFERENCE name, STATEMENT at level 200, at level 70, no associativity) : type_scope.
+Ltac des_ifs := repeat
+  match goal with
+  | |- context[ match ?x with _ => _ end ] =>
+    match (type of x) with
+    | { _ } + { _ } => destruct x
+    | _ => let H_OBS := fresh "H_OBS" in destruct x as [] eqn: H_OBS
+    end
+  | H : context[ match ?x with _ => _ end ] |- _ =>
+    match (type of x) with
+    | { _ } + { _ } => destruct x
+    | _ => let H_OBS := fresh "H_OBS" in destruct x as [] eqn: H_OBS
+    end
+  end.
 
-  Ltac unnw := unfold REFERENCE_HOLDER in *.
+Definition dollar {A : Set} {B : Set} (f : A -> B) (x : A) : B := f x.
 
-  Definition dollar {A : Set} {B : Set} (f : A -> B) (x : A) : B := f x.
+Infix " $ " := dollar (right associativity, at level 100) : program_scope.
 
-  #[global]
-  Infix " $ " := dollar (right associativity, at level 100).
+Class hasEqDec (A : Type) : Type := eq_dec (lhs : A) (rhs : A) : {lhs = rhs} + {lhs <> rhs}.
 
-  Class isSetoid (A : Type) : Type :=
-    { eqProp (lhs : A) (rhs : A) : Prop
-    ; eqProp_Equivalence :> Equivalence eqProp
-    }.
+Definition eqb {A : Type} {hasEqDec : hasEqDec A} (lhs : A) (rhs : A) : bool :=
+  if Prelude.eq_dec lhs rhs then true else false.
 
-  #[global]
-  Infix " == " := eqProp (no associativity, at level 70) : type_scope.
+#[global]
+Instance nat_hasEqDec : hasEqDec nat := Nat.eq_dec.
 
-  #[global, program]
-  Instance arrow_isSetoid {A : Type} {B : Type} (B_isSetoid : isSetoid B) : isSetoid (arrow A B) :=
-    { eqProp (f1 : arrow A B) (f2 : arrow A B) := forall x : A, f1 x == f2 x }.
-  Next Obligation.
-    split.
-    - intros f1 x. reflexivity.
-    - intros f1 f2 f1_eq_f2 x. rewrite f1_eq_f2 with (x := x). reflexivity.
-    - intros f1 f2 f3 f1_eq_f2 f2_eq_f3 x. rewrite f1_eq_f2 with (x := x). rewrite f2_eq_f3 with (x := x). reflexivity.
-  Qed.
+#[global]
+Instance Z_hasEqDec : hasEqDec Z := Z.eq_dec.
 
-  #[global]
-  Instance string_isSetoid : isSetoid string :=
-    { eqProp := @eq string
-    ; eqProp_Equivalence := eq_equivalence
-    }.
+#[global]
+Instance string_hasEqDec : hasEqDec string := string_dec.
 
-  Definition liftRel_option {A : Type} (R : A -> A -> Prop) (lhs : option A) (rhs : option A) : Prop :=
-    match lhs, rhs with
-    | Some lhs', Some rhs' => R lhs' rhs'
-    | None, None => True
-    | _, _ => False
-    end.
+#[global]
+Instance list_hasEqDec {A : Type} (A_hasEqDec : hasEqDec A) : hasEqDec (list A) := @list_eq_dec A A_hasEqDec.
 
-  #[global, program]
-  Instance option_isSetoid {A : Type} (A_isSetoid : isSetoid A) : isSetoid (option A) :=
-    { eqProp := liftRel_option eqProp }.
-  Next Obligation.
-    split.
-    - intros [x | ]; cbn; try tauto.
-      reflexivity.
-    - intros [x | ] [y | ]; cbn; try tauto.
-      intros x_eq_y. symmetry; assumption.
-    - intros [x | ] [y | ] [z | ]; cbn; try tauto.
-      intros x_eq_y y_eq_z. etransitivity; eassumption.
-  Qed.
+Class isSetoid (A : Type) : Type :=
+  { eqProp (lhs : A) (rhs : A) : Prop
+  ; eqProp_Equivalence :> Equivalence eqProp
+  }.
 
-  Lemma option_ext_eq {A : Type} (lhs : option A) (rhs : option A)
-    : lhs = rhs <-> << EXT_EQ : liftRel_option eq lhs rhs >>.
-  Proof. unnw. unfold liftRel_option. destruct lhs as [x | ], rhs as [y | ]; split; try (congruence || tauto). Qed.
+Infix " == " := eqProp (no associativity, at level 70) : type_scope.
 
-  #[global, program]
-  Instance list_isSetoid {A : Type} (A_isSetoid : isSetoid A) : isSetoid (list A) :=
-    { eqProp (lhs : list A) (rhs : list A) := forall i : nat, liftRel_option eqProp (nth_error lhs i) (nth_error rhs i) }.
-  Next Obligation.
-    split.
-    - intros xs i.
-      destruct (nth_error xs i) as [xs_i | ] eqn: OBS_xs_i; cbn in *; try tauto.
-      reflexivity.
-    - intros xs ys xs_eq_ys i. specialize xs_eq_ys with (i := i). 
-      destruct (nth_error xs i) as [xs_i | ] eqn: OBS_xs_i; destruct (nth_error ys i) as [ys_i | ] eqn: OBS_ys_i; cbn in *; try tauto.
-      symmetry; assumption.
-    - intros xs ys zs xs_eq_ys ys_eq_zs i. specialize xs_eq_ys with (i := i). specialize ys_eq_zs with (i := i). 
-      destruct (nth_error xs i) as [xs_i | ] eqn: OBS_xs_i; destruct (nth_error ys i) as [ys_i | ] eqn: OBS_ys_i; cbn in *; destruct (nth_error zs i) as [zs_i | ] eqn: OBS_zs_i; try tauto.
-      etransitivity; eassumption.
-  Qed.
+#[global, program]
+Instance arrow_isSetoid {A : Type} {B : Type} (B_isSetoid : isSetoid B) : isSetoid (arrow A B) :=
+  { eqProp (f1 : arrow A B) (f2 : arrow A B) := forall x : A, f1 x == f2 x }.
+Next Obligation.
+  split.
+  - intros f1 x. reflexivity.
+  - intros f1 f2 f1_eq_f2 x. rewrite f1_eq_f2 with (x := x). reflexivity.
+  - intros f1 f2 f3 f1_eq_f2 f2_eq_f3 x. rewrite f1_eq_f2 with (x := x). rewrite f2_eq_f3 with (x := x). reflexivity.
+Qed.
 
-  Lemma list_ext_eq {A : Type} (lhs : list A) (rhs : list A)
-    : lhs = rhs <-> << EXT_EQ : forall i : nat, liftRel_option eq (nth_error lhs i) (nth_error rhs i) >>.
-  Proof.
-    unnw. split.
-    - intros H_EQ i. rename lhs into xs, rhs into ys. destruct (nth_error xs i) as [xs_i | ] eqn: OBS_xs_i; destruct (nth_error ys i) as [ys_i | ] eqn: OBS_ys_i; cbn in *; try tauto; try congruence.
-    - rename lhs into xs, rhs into ys. revert xs ys. induction xs as [ | x xs IH], ys as [ | y ys]; intros H_EQ; simpl.
-      + reflexivity.
-      + specialize H_EQ with (i := 0). cbn in H_EQ. tauto.
-      + specialize H_EQ with (i := 0). cbn in H_EQ. tauto.
-      + pose proof (H_EQ 0) as x_eq_y. cbn in x_eq_y. specialize (IH ys (fun i : nat => H_EQ (S i))). congruence.
-  Qed.
+#[global]
+Instance string_isSetoid : isSetoid string :=
+  { eqProp := @eq string
+  ; eqProp_Equivalence := eq_equivalence
+  }.
 
-  Class isMonad (M : Type -> Type) : Type :=
-    { pure {A : Type} : A -> M A
-    ; bind {A : Type} {B : Type} : M A -> (A -> M B) -> M B
-    }.
+Definition liftRel_option {A : Type} (R : A -> A -> Prop) (lhs : option A) (rhs : option A) : Prop :=
+  match lhs, rhs with
+  | Some lhs', Some rhs' => R lhs' rhs'
+  | None, None => True
+  | _, _ => False
+  end.
 
-  #[global]
-  Infix " >>= " := bind (left associativity, at level 90).
+#[global, program]
+Instance option_isSetoid {A : Type} (A_isSetoid : isSetoid A) : isSetoid (option A) :=
+  { eqProp := liftRel_option eqProp }.
+Next Obligation.
+  split.
+  - intros [x | ]; cbn; try tauto.
+    reflexivity.
+  - intros [x | ] [y | ]; cbn; try tauto.
+    intros x_eq_y. symmetry; assumption.
+  - intros [x | ] [y | ] [z | ]; cbn; try tauto.
+    intros x_eq_y y_eq_z. etransitivity; eassumption.
+Qed.
 
-  #[global]
-  Instance option_isMonad : isMonad option :=
-    { pure {A} (x : A) := Some x
-    ; bind {A} {B} (m : option A) (k : A -> option B) :=
-      match m with
-      | Some x => k x
-      | None => None
-      end
-    }.
+#[global, program]
+Instance list_isSetoid {A : Type} (A_isSetoid : isSetoid A) : isSetoid (list A) :=
+  { eqProp (lhs : list A) (rhs : list A) := forall i : nat, liftRel_option eqProp (nth_error lhs i) (nth_error rhs i) }.
+Next Obligation.
+  split.
+  - intros xs i.
+    destruct (nth_error xs i) as [xs_i | ] eqn: OBS_xs_i; cbn in *; try tauto.
+    reflexivity.
+  - intros xs ys xs_eq_ys i. specialize xs_eq_ys with (i := i). 
+    destruct (nth_error xs i) as [xs_i | ] eqn: OBS_xs_i; destruct (nth_error ys i) as [ys_i | ] eqn: OBS_ys_i; cbn in *; try tauto.
+    symmetry; assumption.
+  - intros xs ys zs xs_eq_ys ys_eq_zs i. specialize xs_eq_ys with (i := i). specialize ys_eq_zs with (i := i). 
+    destruct (nth_error xs i) as [xs_i | ] eqn: OBS_xs_i; destruct (nth_error ys i) as [ys_i | ] eqn: OBS_ys_i; cbn in *; destruct (nth_error zs i) as [zs_i | ] eqn: OBS_zs_i; try tauto.
+    etransitivity; eassumption.
+Qed.
 
-  #[global]
-  Instance list_isMonad : isMonad list :=
-    { pure {A} (x : A) := [x]
-    ; bind {A} {B} (m : list A) (k : A -> list B) := List.concat (List.map k m)
-    }.
+Class isMonad (M : Type -> Type) : Type :=
+  { pure {A : Type} : A -> M A
+  ; bind {A : Type} {B : Type} : M A -> (A -> M B) -> M B
+  }.
 
-  Class isAlternative (F : Type -> Type) : Type :=
-    { empty {A : Type} : F A
-    ; alt {A : Type} : F A -> F A -> F A
-    }.
+Infix " >>= " := bind (left associativity, at level 90).
 
-  #[global]
-  Infix " <|> " := alt (left associativity, at level 50).
+#[global]
+Instance option_isMonad : isMonad option :=
+  { pure {A} (x : A) := Some x
+  ; bind {A} {B} (m : option A) (k : A -> option B) :=
+    match m with
+    | Some x => k x
+    | None => None
+    end
+  }.
 
-  #[global]
-  Instance option_isAlternative : isAlternative option :=
-    { empty {A} := None
-    ; alt {A} (m1 : option A) (m2 : option A) :=
-      match m1 with
-      | Some x1 => Some x1
-      | None => m2
-      end
-    }.
+#[global]
+Instance list_isMonad : isMonad list :=
+  { pure {A} (x : A) := [x]
+  ; bind {A} {B} (m : list A) (k : A -> list B) := List.concat (List.map k m)
+  }.
 
-  #[global]
-  Instance list_isAlternative : isAlternative list :=
-    { empty {A} := []
-    ; alt {A} (xs1 : list A) (xs2 : list A) := xs1 ++ xs2
-    }.
+Class isAlternative (F : Type -> Type) : Type :=
+  { empty {A : Type} : F A
+  ; alt {A : Type} : F A -> F A -> F A
+  }.
 
-  Fixpoint sequenceM {M : Type -> Type} {M_isMonad : isMonad M} {A : Type} (ms : list (M A)) {struct ms} : M (list A) :=
-    match ms with
-    | [] => pure []
-    | m :: ms' => m >>= fun x => sequenceM ms' >>= fun xs => pure (x :: xs)
-    end.
+Infix " <|> " := alt (left associativity, at level 50).
 
-  Fixpoint sequenceM_ {M : Type -> Type} {M_isMonad : isMonad M} {A : Type} (ms : list (M A)) {struct ms} : M unit :=
-    match ms with
-    | [] => pure tt
-    | m :: ms' => m >>= fun _ => sequenceM_ ms'
-    end.
+#[global]
+Instance option_isAlternative : isAlternative option :=
+  { empty {A} := None
+  ; alt {A} (m1 : option A) (m2 : option A) :=
+    match m1 with
+    | Some x1 => Some x1
+    | None => m2
+    end
+  }.
 
-  Fixpoint lookup {A : Type} {B : Type} (x : A) (eq_dec : forall y : A, {x = y} + {x <> y}) (zs : list (A * B)) : option B :=
-    match zs with
-    | [] => None
-    | (x', y) :: zs' => if eq_dec x' then Some y else lookup x eq_dec zs'
-    end.
+#[global]
+Instance list_isAlternative : isAlternative list :=
+  { empty {A} := []
+  ; alt {A} (xs1 : list A) (xs2 : list A) := xs1 ++ xs2
+  }.
 
-  Definition eq_dec_to_bool {A : Type} (eq_dec : forall lhs : A, forall rhs : A, {lhs = rhs} + {lhs <> rhs}) : A -> A -> bool :=
-    fun lhs : A => fun rhs : A => if eq_dec lhs rhs then true else false.
+Fixpoint sequenceM {M : Type -> Type} {isMonad : isMonad M} {A : Type} (ms : list (M A)) : M (list A) :=
+  match ms with
+  | [] => pure []
+  | m :: ms' => m >>= fun x => sequenceM ms' >>= fun xs => pure (x :: xs)
+  end.
 
-  Lemma lt_strongInd (P : nat -> Prop)
-    (IND : forall n : nat, forall IH : forall m : nat, m < n -> P m, P n)
-    : forall n : nat, P n.
-  Proof.
-    intros n. eapply IND. induction n as [ | n IH].
-    - intros m H_lt. inversion H_lt.
-    - intros m H_lt. eapply IND.
-      intros i i_lt_m. eapply IH. lia.
-  Defined.
+Fixpoint sequenceM_ {M : Type -> Type} {isMonad : isMonad M} {A : Type} (ms : list (M A)) : M unit :=
+  match ms with
+  | [] => pure tt
+  | m :: ms' => m >>= fun _ => sequenceM_ ms'
+  end.
 
-  Lemma acc_lt
-    : forall x : nat, Acc Nat.lt x.
-  Proof. exact (lt_strongInd (@Acc nat Nat.lt) (@Acc_intro nat Nat.lt)). Defined.
+Fixpoint lookup {A : Type} {B : Type} {hasEqDec : hasEqDec A} (x : A) (zs : list (A * B)) : option B :=
+  match zs with
+  | [] => None
+  | (x', y) :: zs' => if Prelude.eqb x x' then Some y else lookup x zs'
+  end.
 
-  Lemma acc_rel {A : Type} {B : Type} (f : A -> B) (R : B -> B -> Prop)
-    (R_wf : forall y : B, Acc R y)
-    : forall x : A, Acc (fun lhs : A => fun rhs : A => R (f lhs) (f rhs)) x.
-  Proof.
-    intros x. remember (f x) as y eqn: y_eq_f_x.
-    revert x y_eq_f_x. induction (R_wf y) as [y' hyp_wf IH].
-    intros x' hyp_eq. econstructor. intros x f_x_R_f_x'.
-    subst y'. eapply IH; [exact (f_x_R_f_x') | reflexivity].
-  Defined.
+Lemma lt_strong_ind (P : nat -> Prop)
+  (IND : forall n : nat, forall IH : forall m : nat, m < n -> P m, P n)
+  : forall n : nat, P n.
+Proof.
+  intros n. eapply IND. induction n as [ | n IH].
+  - intros m H_lt. inversion H_lt.
+  - intros m H_lt. eapply IND.
+    intros i i_lt_m. eapply IH. lia.
+Defined.
 
-  Fixpoint mk_string (xs : list ascii) : string :=
-    match xs with
-    | [] => EmptyString
-    | ch :: xs' => String ch (mk_string xs')
-    end.
+Lemma acc_lt
+  : forall x : nat, Acc Nat.lt x.
+Proof. exact (Prelude.lt_strong_ind (@Acc nat Nat.lt) (@Acc_intro nat Nat.lt)). Defined.
 
-  Section STRING_OPERATIONS.
+Lemma acc_rel {A : Type} {B : Type} (f : A -> B) (R : B -> B -> Prop)
+  (R_wf : forall y : B, Acc R y)
+  : forall x : A, Acc (fun lhs : A => fun rhs : A => R (f lhs) (f rhs)) x.
+Proof.
+  intros x. remember (f x) as y eqn: y_eq_f_x.
+  revert x y_eq_f_x. induction (R_wf y) as [y' hyp_wf IH].
+  intros x' hyp_eq. econstructor. intros x f_x_R_f_x'.
+  subst y'. eapply IH; [exact (f_x_R_f_x') | reflexivity].
+Defined.
 
-  Fixpoint mapFromString {A : Type} (f : ascii -> A) (s : string) {struct s} : list A :=
+Section STRING_OPERATIONS.
+
+Fixpoint mk_string (xs : list char) : string :=
+  match xs with
+  | [] => []%string
+  | ch :: xs' => (ch :: mk_string xs')%string
+  end.
+
+Fixpoint mapFromString {A : Type} (f : char -> A) (s : string) : list A :=
+  match s with
+  | []%string => []
+  | (ch :: s')%string => f ch :: mapFromString f s'
+  end.
+
+Fixpoint String_take (n : nat) (s : string) : string :=
+  match n with
+  | O => []%string
+  | S n' =>
     match s with
-    | EmptyString => []
-    | String ch s' => f ch :: mapFromString f s'
-    end.
+    | []%string => []%string
+    | (ch :: s')%string => (ch :: String_take n' s')%string
+    end
+  end.
 
-  Fixpoint String_take (n : nat) (s : string) {struct n} : string :=
-    match n with
-    | O => EmptyString
-    | S n' =>
-      match s with
-      | EmptyString => EmptyString
-      | String ch s' => String ch (String_take n' s')
-      end
-    end.
+Fixpoint String_concat (ss : list string) : string :=
+  match ss with
+  | [] => ""%string
+  | s :: ss' => (s ++ String_concat ss')%string
+  end.
 
-  Fixpoint String_concat (ss : list string) {struct ss} : string :=
-    match ss with
-    | [] => ""%string
-    | s :: ss' => (s ++ String_concat ss')%string
-    end.
-
-  Fixpoint String_drop (n : nat) (s : string) {struct n} : string :=
-    match n with
-    | O => s
-    | S n' =>
-      match s with
-      | EmptyString => EmptyString
-      | String ch s' => String_drop n' s'
-      end
-    end.
-
-  Fixpoint String_rev (s : string) {struct s} : string :=
+Fixpoint String_drop (n : nat) (s : string) : string :=
+  match n with
+  | O => s
+  | S n' =>
     match s with
-    | EmptyString => EmptyString
-    | String ch s' => (String_rev s' ++ String ch EmptyString)%string
-    end.
+    | []%string => []%string
+    | (ch :: s')%string => String_drop n' s'
+    end
+  end.
 
-  #[program]
-  Fixpoint nat_to_string' (n : nat) (s : string) {measure n} : string :=
-    let ch : ascii :=
-      match n mod 10 with
-      | 1 => "1"%char
-      | 2 => "2"%char
-      | 3 => "3"%char
-      | 4 => "4"%char
-      | 5 => "5"%char
-      | 6 => "6"%char
-      | 7 => "7"%char
-      | 8 => "8"%char
-      | 9 => "9"%char
-      | _ => "0"%char
-      end
-    in
-    if Nat.eq_dec n 0 then s else nat_to_string' (n / 10) (String ch s).
-  Next Obligation. lia. Defined.
-  Next Obligation. lia. Defined.
-  Next Obligation. change (n / 10 < n). pose proof (Nat.div_mod n 10). pose proof (Nat.mod_bound_pos n 10). lia. Defined.
+Fixpoint String_rev (s : string) : string :=
+  match s with
+  | []%string => []%string
+  | (ch :: s')%string => (String_rev s' ++ (ch :: []))%string
+  end.
 
-  Definition nat_to_string (n : nat) : string := if Nat.eqb n 0 then "0"%string else nat_to_string' n ""%string.
+Definition showDigit (n : nat) : char :=
+  match n with
+  | 0 => "0"%char
+  | 1 => "1"%char
+  | 2 => "2"%char
+  | 3 => "3"%char
+  | 4 => "4"%char
+  | 5 => "5"%char
+  | 6 => "6"%char
+  | 7 => "7"%char
+  | 8 => "8"%char
+  | 9 => "9"%char
+  | _ => "_"%char
+  end.
 
-  Definition Z_to_string (z : Z) : string :=
-    match z with
-    | Z0 => "0"%string
-    | Zpos pos => nat_to_string (Pos.to_nat pos)
-    | Zneg neg => ("-" ++ nat_to_string (Pos.to_nat neg))%string
-    end.
+#[program]
+Fixpoint nat_to_string1 (n : nat) (s : string) {measure n} : string :=
+  if Prelude.eq_dec n 0 then s else nat_to_string1 (n / 10) (showDigit (n mod 10) :: s)%string.
+Next Obligation. change (n / 10 < n). pose proof (Nat.div_mod n 10). pose proof (Nat.mod_bound_pos n 10). lia. Defined.
 
-  Fixpoint nat_from_string' (s : string) (n : nat) : nat :=
-    match s with
-    | EmptyString => n
-    | String "1"%char s' => nat_from_string' s' (n * 10 + 1)
-    | String "2"%char s' => nat_from_string' s' (n * 10 + 2)
-    | String "3"%char s' => nat_from_string' s' (n * 10 + 3)
-    | String "4"%char s' => nat_from_string' s' (n * 10 + 4)
-    | String "5"%char s' => nat_from_string' s' (n * 10 + 5)
-    | String "6"%char s' => nat_from_string' s' (n * 10 + 6)
-    | String "7"%char s' => nat_from_string' s' (n * 10 + 7)
-    | String "8"%char s' => nat_from_string' s' (n * 10 + 8)
-    | String "9"%char s' => nat_from_string' s' (n * 10 + 9)
-    | String _ s' => nat_from_string' s' (n * 10)
-    end.
+Lemma nat_to_string1_unfold (n : nat) (s : string) :
+  nat_to_string1 n s =
+  if Prelude.eq_dec n 0 then s else nat_to_string1 (n / 10) (showDigit (n mod 10) :: s)%string.
+Proof.
+  unfold nat_to_string1 at 1. unfold nat_to_string1_func.
+  rewrite WfExtensionality.fix_sub_eq_ext. simpl.
+  destruct (Prelude.eq_dec n 0) as [H_yes | H_no]; reflexivity.
+Qed.
 
-  Definition nat_from_string (s : string) : nat := nat_from_string' s 0.
+Definition nat_to_string (n : nat) : string :=
+  if Nat.eqb n 0 then "0"%string else nat_to_string1 n ""%string.
 
-  Lemma String_app_assoc (s1 : string) (s2 : string) (s3 : string)
-    : ((s1 ++ s2) ++ s3)%string = (s1 ++ (s2 ++ s3))%string.
-  Proof.
-    revert s2 s3. induction s1 as [ | ch1 s1 IH]; simpl; intros.
-    - reflexivity.
-    - eapply f_equal. eauto.
-  Qed.
+Definition Z_to_string (z : Z) : string :=
+  match z with
+  | Z0 => "0"%string
+  | Zpos pos => nat_to_string (Pos.to_nat pos)
+  | Zneg neg => ("-" ++ nat_to_string (Pos.to_nat neg))%string
+  end.
 
-  Lemma String_app_nil_l (s1 : string)
-    : (s1 ++ "")%string = s1.
-  Proof. induction s1 as [ | ch1 s1 IH]; simpl; congruence. Qed.
+Fixpoint nat_from_string1 (n : nat) (s : string) : nat :=
+  match s with
+  | ("0" :: s')%string => nat_from_string1 (n * 10 + 0) s'
+  | ("1" :: s')%string => nat_from_string1 (n * 10 + 1) s'
+  | ("2" :: s')%string => nat_from_string1 (n * 10 + 2) s'
+  | ("3" :: s')%string => nat_from_string1 (n * 10 + 3) s'
+  | ("4" :: s')%string => nat_from_string1 (n * 10 + 4) s'
+  | ("5" :: s')%string => nat_from_string1 (n * 10 + 5) s'
+  | ("6" :: s')%string => nat_from_string1 (n * 10 + 6) s'
+  | ("7" :: s')%string => nat_from_string1 (n * 10 + 7) s'
+  | ("8" :: s')%string => nat_from_string1 (n * 10 + 8) s'
+  | ("9" :: s')%string => nat_from_string1 (n * 10 + 9) s'
+  | _ => n
+  end.
 
-  Lemma String_app_nil_r (s1 : string)
-    : ("" ++ s1)%string = s1.
-  Proof. reflexivity. Qed.
+Definition nat_from_string (s : string) : nat := nat_from_string1 0 s.
 
-  Lemma String_app_length (s1 : string) (s2 : string)
-    : length (s1 ++ s2)%string = length s1 + length s2.
-  Proof. induction s1 as [ | ch1 s1]; simpl; lia. Qed.
+End STRING_OPERATIONS.
 
-  Lemma String_take_app_String_drop (n : nat) (s : string)
-    (n_lt_length_s : n < length s)
-    : (String_take n s ++ String_drop n s)%string = s.
-  Proof.
-    revert s n_lt_length_s. induction n as [ | n IH].
-    - intros s _. reflexivity.
-    - intros s n_lt_length_s. destruct s as [ | ch s'].
-      + reflexivity.
-      + simpl. eapply f_equal. eapply IH. simpl in n_lt_length_s. lia.
-  Qed.
+Definition isNum (ch : char) : bool := Ascii.leb "0"%char ch && Ascii.leb ch "9"%char.
 
-  Lemma String_rev_app (s1 : string) (s2 : string)
-    : String_rev (s1 ++ s2)%string = (String_rev s2 ++ String_rev s1)%string.
-  Proof.
-    induction s1 as [ | ch1 s1 IH]; simpl.
-    - rewrite String_app_nil_l. reflexivity.
-    - rewrite IH. eapply String_app_assoc.
-  Qed.
+Definition isLower (ch : char) : bool := Ascii.leb "a"%char ch && Ascii.leb ch "z"%char.
 
-  Lemma String_rev_involute (s : string)
-    : String_rev (String_rev s) = s.
-  Proof.
-    induction s as [ | ch s IH]; simpl.
-    - reflexivity.
-    - rewrite String_rev_app, IH. reflexivity.
-  Qed.
+Definition isUpper (ch : char) : bool := Ascii.leb "A"%char ch && Ascii.leb ch "Z"%char.
 
-  Lemma String_rev_ind (phi : string -> Prop)
-    (H_EmptyString : phi EmptyString)
-    (H_String : forall ch : ascii, forall s : string, phi s -> phi (s ++ String ch EmptyString)%string)
-    : forall s : string, phi s.
-  Proof.
-    intros s. rewrite <- String_rev_involute with (s := s).
-    generalize (String_rev s). clear s. induction s as [ | ch s IH]; simpl.
-    - eapply H_EmptyString.
-    - eapply H_String. exact (IH).
-  Qed.
+Definition isAlpha (ch : char) : bool := isLower ch || isUpper ch.
 
-  Lemma String_rev_dual (phi : string -> Prop)
-    (H_rev : forall s : string, phi (String_rev s))
-    : forall s : string, phi s.
-  Proof.
-    induction s as [ | ch s _] using String_rev_ind.
-    - eapply H_rev with (s := ""%string).
-    - rewrite <- String_rev_involute with (s := s).
-      eapply H_rev with (s := String ch (String_rev s)).
-  Qed.
-
-  Lemma String_rev_inj (s1 : string) (s2 : string)
-    (REV_EQ : String_rev s1 = String_rev s2)
-    : s1 = s2.
-  Proof.
-    rewrite <- String_rev_involute with (s := s1).
-    rewrite <- String_rev_involute with (s := s2).
-    eapply f_equal. eassumption.
-  Qed.
-
-  Lemma String_cancel_l (s1 : string) (s2 : string) (s3 : string)
-    (s1_app_s2_eq_s1_app_s3 : (s1 ++ s2)%string = (s1 ++ s3)%string)
-    : s2 = s3.
-  Proof.
-    revert s2 s3 s1_app_s2_eq_s1_app_s3. induction s1 as [ | ch1 s1 IH]; simpl; intros.
-    - eauto.
-    - inversion s1_app_s2_eq_s1_app_s3. eauto.
-  Qed.
-
-  Lemma String_cancel_r (s1 : string) (s2 : string) (s3 : string)
-    (s1_app_s3_eq_s2_app_s3 : (s1 ++ s3)%string = (s2 ++ s3)%string)
-    : s1 = s2.
-  Proof.
-    revert s2 s3 s1_app_s3_eq_s2_app_s3. pattern s1. revert s1. eapply String_rev_dual.
-    intros s1 s2. pattern s2. revert s2. eapply String_rev_dual.
-    intros s2 s3. pattern s3. revert s3. eapply String_rev_dual.
-    intros s3. do 2 rewrite <- String_rev_app.
-    intros REV_EQ. apply String_rev_inj, String_cancel_l in REV_EQ. congruence. 
-  Qed.
-
-  End STRING_OPERATIONS.
+Definition isAlphaNum (ch : char) : bool := isAlpha ch || isNum ch.
 
 End Prelude.
 
 Export Prelude.
 
+Module PreludeTheory.
+
+Import StringNotations ListNotations.
+
+Lemma eqb_eq {A : Type} {hasEqDec : Prelude.hasEqDec A} (lhs : A) (rhs : A)
+  : Prelude.eqb lhs rhs = true <-> lhs = rhs.
+Proof.
+  unfold Prelude.eqb. destruct (Prelude.eq_dec lhs rhs) as [H_yes | H_no].
+  - split; [intros _; exact (H_yes) | intros _; reflexivity].
+  - split; [intros H_false; inversion H_false | intros H_false; contradiction (H_no H_false)].
+Qed.
+
+Lemma eqb_neq {A : Type} {hasEqDec : Prelude.hasEqDec A} (lhs : A) (rhs : A)
+  : Prelude.eqb lhs rhs = false <-> lhs <> rhs.
+Proof.
+  unfold Prelude.eqb. destruct (Prelude.eq_dec lhs rhs) as [H_yes | H_no].
+  - split; [intros H_false; inversion H_false | intros H_false; contradiction (H_false H_yes)].
+  - split; [intros _; exact (H_no) | intros _; reflexivity].
+Qed.
+
+Lemma option_ext_eq {A : Type} (lhs : option A) (rhs : option A)
+  : lhs = rhs <-> << EXT_EQ : liftRel_option eq lhs rhs >>.
+Proof. unnw. unfold liftRel_option. destruct lhs as [x | ], rhs as [y | ]; split; try (congruence || tauto). Qed.
+
+Lemma list_ext_eq {A : Type} (lhs : list A) (rhs : list A)
+  : lhs = rhs <-> << EXT_EQ : forall i : nat, liftRel_option eq (nth_error lhs i) (nth_error rhs i) >>.
+Proof.
+  unnw. split.
+  - intros H_EQ i. rename lhs into xs, rhs into ys. destruct (nth_error xs i) as [xs_i | ] eqn: OBS_xs_i; destruct (nth_error ys i) as [ys_i | ] eqn: OBS_ys_i; cbn in *; try tauto; try congruence.
+  - rename lhs into xs, rhs into ys. revert xs ys. induction xs as [ | x xs IH], ys as [ | y ys]; intros H_EQ; simpl.
+    + reflexivity.
+    + specialize H_EQ with (i := 0). cbn in H_EQ. tauto.
+    + specialize H_EQ with (i := 0). cbn in H_EQ. tauto.
+    + pose proof (H_EQ 0) as x_eq_y. cbn in x_eq_y. specialize (IH ys (fun i : nat => H_EQ (S i))). congruence.
+Qed.
+
+Lemma fold_left_ind {A : Type} {B : Type} (phi : A -> Prop) (f : A -> B -> A) (z0 : A) (xs : list B)
+  (phi_z0 : phi z0)
+  (phi_f_z_x_if_phi_z : forall z : A, forall x : B, << IH : phi z >> -> phi (f z x))
+  : phi (fold_left f xs z0).
+Proof.
+  unnw. revert xs z0 phi_z0. induction xs as [ | x xs IH]; simpl; intros z phi_z.
+  - exact (phi_z).
+  - eapply IH with (z0 := f z x). eapply phi_f_z_x_if_phi_z with (z := z) (x := x). exact (phi_z).
+Defined.
+
+Lemma String_app_assoc (s1 : string) (s2 : string) (s3 : string)
+  : ((s1 ++ s2) ++ s3)%string = (s1 ++ (s2 ++ s3))%string.
+Proof.
+  revert s2 s3. induction s1 as [ | ch1 s1 IH]; simpl; intros.
+  - reflexivity.
+  - eapply f_equal. eauto.
+Qed.
+
+Lemma String_app_nil_l (s1 : string)
+  : ("" ++ s1)%string = s1.
+Proof. reflexivity. Qed.
+
+Lemma String_app_nil_r (s1 : string)
+  : (s1 ++ "")%string = s1.
+Proof. induction s1 as [ | ch1 s1 IH]; simpl; congruence. Qed.
+
+Lemma String_app_length (s1 : string) (s2 : string)
+  : length (s1 ++ s2)%string = length s1 + length s2.
+Proof. induction s1 as [ | ch1 s1]; simpl; lia. Qed.
+
+Lemma String_take_ge_length (n : nat) (s : string)
+  (n_ge_length : n >= length s)
+  : String_take n s = s.
+Proof.
+  revert n s n_ge_length. induction n as [ | n IH], s as [ | ch s]; simpl; intros ?.
+  - reflexivity.
+  - lia.
+  - reflexivity.
+  - eapply f_equal. eapply IH. lia.
+Qed.
+
+Lemma String_drop_ge_length (n : nat) (s : string)
+  (n_ge_length : n >= length s)
+  : String_drop n s = []%string.
+Proof.
+  revert n s n_ge_length. induction n as [ | n IH], s as [ | ch s]; simpl; intros ?.
+  - reflexivity.
+  - lia.
+  - reflexivity.
+  - eapply IH. lia.
+Qed.
+
+Lemma String_take_app_String_drop (n : nat) (s : string)
+  : (String_take n s ++ String_drop n s)%string = s.
+Proof.
+  assert (n < length s \/ n >= length s) as [n_lt_length_s | n_ge_length] by lia.
+  - revert s n_lt_length_s. induction n as [ | n IH].
+    + intros s _. reflexivity.
+    + intros s n_lt_length_s. destruct s as [ | ch s'].
+      * reflexivity.
+      * simpl. eapply f_equal. eapply IH. simpl in n_lt_length_s. lia.
+  - rewrite String_take_ge_length; trivial.
+    rewrite String_drop_ge_length; trivial.
+    eapply String_app_nil_r.
+Qed.
+
+Lemma String_rev_app (s1 : string) (s2 : string)
+  : String_rev (s1 ++ s2)%string = (String_rev s2 ++ String_rev s1)%string.
+Proof.
+  induction s1 as [ | ch1 s1 IH]; simpl.
+  - rewrite String_app_nil_r. reflexivity.
+  - rewrite IH. eapply String_app_assoc.
+Qed.
+
+Lemma String_rev_involute (s : string)
+  : String_rev (String_rev s) = s.
+Proof.
+  induction s as [ | ch s IH]; simpl.
+  - reflexivity.
+  - rewrite String_rev_app, IH. reflexivity.
+Qed.
+
+Lemma String_rev_ind (phi : string -> Prop)
+  (H_EmptyString : phi []%string)
+  (H_String : forall ch : ascii, forall s : string, phi s -> phi (s ++ (ch :: [])%string)%string)
+  : forall s : string, phi s.
+Proof.
+  intros s. rewrite <- String_rev_involute with (s := s).
+  generalize (String_rev s). clear s. induction s as [ | ch s IH]; simpl.
+  - eapply H_EmptyString%string.
+  - eapply H_String. exact (IH).
+Qed.
+
+Lemma String_rev_dual (phi : string -> Prop)
+  (H_rev : forall s : string, phi (String_rev s))
+  : forall s : string, phi s.
+Proof.
+  induction s as [ | ch s _] using String_rev_ind.
+  - eapply H_rev with (s := []%string).
+  - rewrite <- String_rev_involute with (s := s).
+    eapply H_rev with (s := (ch :: String_rev s)%string).
+Qed.
+
+Lemma String_rev_inj (s1 : string) (s2 : string)
+  (REV_EQ : String_rev s1 = String_rev s2)
+  : s1 = s2.
+Proof.
+  rewrite <- String_rev_involute with (s := s1).
+  rewrite <- String_rev_involute with (s := s2).
+  eapply f_equal. eassumption.
+Qed.
+
+Lemma String_cancel_l (s1 : string) (s2 : string) (s3 : string)
+  (s1_app_s2_eq_s1_app_s3 : (s1 ++ s2)%string = (s1 ++ s3)%string)
+  : s2 = s3.
+Proof.
+  revert s2 s3 s1_app_s2_eq_s1_app_s3. induction s1 as [ | ch1 s1 IH]; simpl; intros.
+  - eauto.
+  - inversion s1_app_s2_eq_s1_app_s3. eauto.
+Qed.
+
+Lemma String_cancel_r (s1 : string) (s2 : string) (s3 : string)
+  (s1_app_s3_eq_s2_app_s3 : (s1 ++ s3)%string = (s2 ++ s3)%string)
+  : s1 = s2.
+Proof.
+  revert s2 s3 s1_app_s3_eq_s2_app_s3. pattern s1. revert s1. eapply String_rev_dual.
+  intros s1 s2. pattern s2. revert s2. eapply String_rev_dual.
+  intros s2 s3. pattern s3. revert s3. eapply String_rev_dual.
+  intros s3. do 2 rewrite <- String_rev_app.
+  intros REV_EQ. apply String_rev_inj, String_cancel_l in REV_EQ. congruence.
+Qed.
+
+End PreludeTheory.
+
 Module P.
 
-  Import ListNotations.
+Import StringNotations ListNotations.
 
-  Definition parserT (M : Type -> Type) (A : Type) : Type := string -> M (A * string)%type.
+Definition parserT (M : Type -> Type) (A : Type) : Type := string -> M (A * string)%type.
 
-  #[global]
-  Instance parserT_isMonad {M : Type -> Type} (M_isMonad : isMonad M) : isMonad (parserT M) :=
-    { pure {A} := curry pure
-    ; bind {A} {B} (m : parserT M A) (k : A -> parserT M B) := fun s : string => m s >>= uncurry k
-    }.
+#[global]
+Instance parserT_isMonad {M : Type -> Type} (M_isMonad : isMonad M) : isMonad (parserT M) :=
+  { pure {A} := curry pure
+  ; bind {A} {B} (m : parserT M A) (k : A -> parserT M B) := fun s : string => m s >>= uncurry k
+  }.
 
-  #[global]
-  Instance parserT_isAlternative {M : Type -> Type} (M_isAlternative : isAlternative M) : isAlternative (parserT M) :=
-    { empty {A} := fun s : string => empty
-    ; alt {A} (p1 : parserT M A) (p2 : parserT M A) := fun s : string => p1 s <|> p2 s
-    }.
+#[global]
+Instance parserT_isAlternative {M : Type -> Type} (M_isAlternative : isAlternative M) : isAlternative (parserT M) :=
+  { empty {A} := fun s : string => empty
+  ; alt {A} (p1 : parserT M A) (p2 : parserT M A) := fun s : string => p1 s <|> p2 s
+  }.
 
-  Definition parser : Type -> Type := parserT option.
+Definition parser : Type -> Type := parserT option.
 
-  Definition eqP {A : Type} (lhs : parser A) (rhs : parser A) : Prop := forall s : string, lhs s = rhs s.
+Definition eqP {A : Type} (lhs : parser A) (rhs : parser A) : Prop := forall s : string, lhs s = rhs s.
 
-  #[global]
-  Instance eqP_Equivalence {A : Type}
-    : Equivalence (@eqP A).
-  Proof.
-    split.
-    - intros x s. reflexivity.
-    - intros x y x_eq_y s. rewrite x_eq_y with (s := s). reflexivity.
-    - intros x y z x_eq_y y_eq_z s. rewrite x_eq_y with (s := s). rewrite y_eq_z with (s := s). reflexivity.
-  Qed.
+#[global]
+Instance eqP_Equivalence {A : Type}
+  : Equivalence (@eqP A).
+Proof.
+  split.
+  - intros x s. reflexivity.
+  - intros x y x_eq_y s. rewrite x_eq_y with (s := s). reflexivity.
+  - intros x y z x_eq_y y_eq_z s. rewrite x_eq_y with (s := s). rewrite y_eq_z with (s := s). reflexivity.
+Qed.
 
-  #[global]
-  Instance parser_isSetoid {A : Type} : isSetoid (parser A) :=
-    { eqProp := eqP
-    ; eqProp_Equivalence := eqP_Equivalence
-    }.
+#[global]
+Instance parser_isSetoid {A : Type} : isSetoid (parser A) :=
+  { eqProp := @eqP A
+  ; eqProp_Equivalence := @eqP_Equivalence A
+  }.
 
-  #[global]
-  Add Parametric Morphism {A : Type} {B : Type}
-    : (@bind parser (parserT_isMonad option_isMonad) A B) with signature (eqProp (isSetoid := parser_isSetoid) ==> eqProp (isSetoid := arrow_isSetoid parser_isSetoid) ==> eqProp (isSetoid := parser_isSetoid)) as bind_lifts_eqP.
-  Proof. intros m1 m2 m1_eq_m2 k1 k2 k1_eq_k2 s. simpl. rewrite m1_eq_m2 with (s := s). destruct (m2 s) as [[x s'] | ]; simpl; trivial. eapply k1_eq_k2. Qed.
+#[global]
+Add Parametric Morphism {A : Type} {B : Type}
+  : (@bind parser (parserT_isMonad option_isMonad) A B) with signature (eqProp (isSetoid := parser_isSetoid) ==> eqProp (isSetoid := arrow_isSetoid parser_isSetoid) ==> eqProp (isSetoid := parser_isSetoid)) as bind_lifts_eqP.
+Proof. intros m1 m2 m1_eq_m2 k1 k2 k1_eq_k2 s. simpl. rewrite m1_eq_m2 with (s := s). destruct (m2 s) as [[x s'] | ]; simpl; trivial. eapply k1_eq_k2. Qed.
 
-  Lemma bind_assoc {A : Type} {B : Type} {C : Type} (m0 : parser A) (k1 : A -> parser B) (k2 : B -> parser C)
-    : ((m0 >>= k1) >>= k2) == (m0 >>= fun x => (k1 x >>= k2)).
-  Proof. intros s. simpl. destruct (m0 s) as [[x s'] | ]; reflexivity. Qed.
+Lemma bind_assoc {A : Type} {B : Type} {C : Type} (m0 : parser A) (k1 : A -> parser B) (k2 : B -> parser C)
+  : ((m0 >>= k1) >>= k2) == (m0 >>= fun x => (k1 x >>= k2)).
+Proof. intros s. simpl. destruct (m0 s) as [[x s'] | ]; reflexivity. Qed.
 
-  Lemma bind_pure_l {A : Type} {B : Type} (x : A) (k : A -> parser B)
-    : (pure x >>= k) == k x.
-  Proof. intros s. simpl. reflexivity. Qed.
+Lemma bind_pure_l {A : Type} {B : Type} (x : A) (k : A -> parser B)
+  : (pure x >>= k) == k x.
+Proof. intros s. simpl. reflexivity. Qed.
 
-  Lemma bind_pure_r {A : Type} (m : parser A)
-    : (m >>= pure) == m.
-  Proof. intros s. simpl. destruct (m s) as [[x s'] | ]; reflexivity. Qed.
+Lemma bind_pure_r {A : Type} (m : parser A)
+  : (m >>= pure) == m.
+Proof. intros s. simpl. destruct (m s) as [[x s'] | ]; reflexivity. Qed.
 
-  #[global]
-  Add Parametric Morphism {A : Type}
-    : (@alt parser (parserT_isAlternative option_isAlternative) A) with signature (eqProp (isSetoid := parser_isSetoid) ==> eqProp (isSetoid := parser_isSetoid) ==> eqProp (isSetoid := parser_isSetoid)) as alt_lifts_eqP.
-  Proof. intros lhs1 rhs1 lhs1_eq_rhs1 lhs2 rhs2 lhs2_eq_rhs2 s. simpl. rewrite lhs1_eq_rhs1 with (s := s). rewrite lhs2_eq_rhs2 with (s := s). reflexivity. Qed.
+#[global]
+Add Parametric Morphism {A : Type}
+  : (@alt parser (parserT_isAlternative option_isAlternative) A) with signature (eqProp (isSetoid := parser_isSetoid) ==> eqProp (isSetoid := parser_isSetoid) ==> eqProp (isSetoid := parser_isSetoid)) as alt_lifts_eqP.
+Proof. intros lhs1 rhs1 lhs1_eq_rhs1 lhs2 rhs2 lhs2_eq_rhs2 s. simpl. rewrite lhs1_eq_rhs1 with (s := s). rewrite lhs2_eq_rhs2 with (s := s). reflexivity. Qed.
 
-  Lemma alt_assoc {A : Type} (m1 : parser A) (m2 : parser A) (m3 : parser A)
-    : (m1 <|> m2) <|> m3 == m1 <|> (m2 <|> m3).
-  Proof. intros s. simpl. destruct (m1 s) as [[x1 s'] | ]; reflexivity. Qed.
+Lemma alt_assoc {A : Type} (p1 : parser A) (p2 : parser A) (p3 : parser A)
+  : (p1 <|> p2) <|> p3 == p1 <|> (p2 <|> p3).
+Proof. intros s. simpl. destruct (p1 s) as [[x1 s'] | ]; reflexivity. Qed.
 
-  Lemma alt_empty_l {A : Type} (m : parser A)
-    : empty <|> m == m.
-  Proof. intros s. simpl. reflexivity. Qed.
+Lemma alt_empty_l {A : Type} (p : parser A)
+  : empty <|> p == p.
+Proof. intros s. simpl. reflexivity. Qed.
 
-  Lemma alt_empty_r {A : Type} (m : parser A)
-    : m <|> empty == m.
-  Proof. intros s. simpl. destruct (m s) as [[x s'] | ]; reflexivity. Qed.
+Lemma alt_empty_r {A : Type} (p : parser A)
+  : p <|> empty == p.
+Proof. intros s. simpl. destruct (p s) as [[x s'] | ]; reflexivity. Qed.
 
-  Definition isLt {A : Type} (p : parser A) : Prop :=
-    forall s : string,
-    match p s with
-    | Some (x, s') => length s' < length s
-    | None => True
-    end.
+Definition string_wf : forall s : string, Acc (fun s1 : string => fun s2 : string => length s1 < length s2) s :=
+  Prelude.acc_rel String.length Nat.lt Prelude.acc_lt.
 
-  Definition isLe {A : Type} (p : parser A) : Prop :=
-    forall s : string,
-    match p s with
-    | Some (x, s') => length s' <= length s
-    | None => True
-    end.
+Definition isLt {A : Type} (p : parser A) : Prop :=
+  forall s : string,
+  match p s with
+  | Some (x, s') => length s' < length s
+  | None => True
+  end.
 
-  Section PARSER_COMBINATORS.
+Definition isLe {A : Type} (p : parser A) : Prop :=
+  forall s : string,
+  match p s with
+  | Some (x, s') => length s' <= length s
+  | None => True
+  end.
 
-  Definition satisfyP (cond : ascii -> bool) : parser ascii :=
-    fun s : string =>
-    match s with
-    | EmptyString => None
-    | String ch s' => if cond ch then Some (ch, s') else None
-    end.
+Lemma isLt_implies_isLe {A : Type} (p : parser A)
+  (p_isLt : isLt p)
+  : isLe p.
+Proof.
+  intros s. pose proof (p_isLt s) as H.
+  destruct (p s) as [[x s'] | ]; trivial. lia.
+Qed.
 
-  Lemma satisfyP_isLt (cond : ascii -> bool)
-    : isLt (satisfyP cond).
-  Proof.
-    intros s. unfold satisfyP. destruct s as [ | ch s']; trivial.
-    destruct (cond ch); trivial. simpl. red. reflexivity.
-  Qed.
+#[global]
+Add Parametric Morphism {A : Type}
+  : (@isLt A) with signature (eqProp ==> iff) as isLt_compatWith_eqP.
+Proof.
+  assert (claim : forall p1 : parser A, forall p2 : parser A, p1 == p2 -> isLt p1 -> isLt p2).
+  { intros p1 p2 p1_eq_p2 p1_isLt s. rewrite <- p1_eq_p2 with (s := s). exact (p1_isLt s). }
+  intros p1 p2 p1_eq_p2; split; [intros p1_isLt | intros p2_isLt; symmetry in p1_eq_p2]; eauto.
+Qed.
 
-  Definition stringP : string -> parser unit := sequenceM_ ∘ mapFromString (satisfyP ∘ Ascii.eqb).
+#[global]
+Add Parametric Morphism {A : Type}
+  : (@isLe A) with signature (eqProp ==> iff) as isLe_compatWith_eqP.
+Proof.
+  assert (claim : forall p1 : parser A, forall p2 : parser A, p1 == p2 -> isLe p1 -> isLe p2).
+  { intros p1 p2 p1_eq_p2 p1_isLe s. rewrite <- p1_eq_p2 with (s := s). exact (p1_isLe s). }
+  intros p1 p2 p1_eq_p2; split; [intros p1_isLe | intros p2_isLe; symmetry in p1_eq_p2]; eauto.
+Qed.
 
-  Lemma stringP_isLt (str : string)
-    (length_str_gt_0 : length str > 0)
-    : isLt (stringP str).
-  Proof.
-    enough (to_show : length str = 0 \/ isLt (stringP str)).
-    { destruct to_show; [lia | assumption]. }
-    clear length_str_gt_0. induction str as [ | ch str IH_str].
-    - left. reflexivity.
-    - simpl. right. intros s.
-      assert (H_Acc : Acc (fun s1 : string => fun s2 : string => length s1 < length s2) s) by exact (Prelude.acc_rel String.length lt Prelude.acc_lt s).
-      revert ch str IH_str. induction H_Acc as [s _ IH]. intros. simpl.
-      red. red. simpl. red. pose proof (satisfyP_isLt (Ascii.eqb ch) s) as length_s_gt_length_s'.
-      destruct (satisfyP (Ascii.eqb ch) s) as [[x s'] | ] eqn: H_OBS; trivial.
-      simpl. specialize (IH s' length_s_gt_length_s'). destruct str as [ | ch' str'].
-      + assert (IH_claim : length "" = 0 \/ isLt (stringP "")) by now left.
-        specialize (IH ch EmptyString IH_claim). do 2 red in IH. simpl in IH. red in IH. simpl. assumption.
-      + assert (IH_claim : length (String ch' str') = 0 \/ isLt (stringP (String ch' str'))).
-        { right. destruct IH_str as [IH_str | IH_str]; [inversion IH_str | assumption]. }
-        specialize (IH ch (String ch' str') IH_claim). do 2 red in IH. simpl in IH. red in IH.
-        destruct IH_str as [IH_str | IH_str].
-        * inversion IH_str.
-        * specialize (IH_str s'). red in IH_str. red in IH_str.
-          destruct (sequenceM_ (mapFromString (satisfyP ∘ Ascii.eqb) (String ch' str')) s') as [[x' s''] | ] eqn: H_OBS'; trivial. lia.
-  Qed.
+Lemma bind_m_k_isLt_if_m_isLt_and_k_isLe {A : Type} {B : Type} (m : parser A) (k : A -> parser B)
+  (m_isLt : isLt m)
+  (k_isLe : forall x : A, isLe (k x))
+  : isLt (bind (A := A) (B := B) m k).
+Proof.
+  intros s. pose proof (m_isLt s) as H0.
+  simpl. destruct (m s) as [[x' s'] | ]; trivial.
+  simpl. pose proof (k_isLe x' s') as H1.
+  destruct (k x' s') as [[x'' s''] | ]; trivial. lia.
+Qed.
 
-  #[program]
-  Fixpoint someP {A : Type} (p : parser A) (p_isLt : isLt p) (s : string) {measure (length s)} : option (list A * string) :=
-    match p s with
-    | None => None
-    | Some (x, s') =>
-      match someP p p_isLt s' with
-      | None => Some ([x], s')
-      | Some (xs, s'') => Some (x :: xs, s'')
-      end
-    end.
-  Next Obligation. pose proof (p_isLt s) as H. rewrite <- Heq_anonymous in H. assumption. Defined.
+Lemma bind_m_k_isLt_if_m_isLe_and_k_isLt {A : Type} {B : Type} (m : parser A) (k : A -> parser B)
+  (m_isLe : isLe m)
+  (k_isLt : forall x : A, isLt (k x))
+  : isLt (bind (A := A) (B := B) m k).
+Proof.
+  intros s. pose proof (m_isLe s) as H0.
+  simpl. destruct (m s) as [[x' s'] | ]; trivial.
+  simpl. pose proof (k_isLt x' s') as H1.
+  destruct (k x' s') as [[x'' s''] | ]; trivial. lia.
+Qed.
 
-  Example someP_example1
-    : (someP (satisfyP (fun ch : ascii => true)) (satisfyP_isLt _) "abc"%string)
-    = Some (["a"%char; "b"%char; "c"%char], ""%string).
-  Proof. reflexivity. Qed.
+Lemma bind_m_k_isLe_if_m_isLe_and_k_isLe {A : Type} {B : Type} (m : parser A) (k : A -> parser B)
+  (m_isLe : isLe m)
+  (k_isLe : forall x : A, isLe (k x))
+  : isLe (bind (A := A) (B := B) m k).
+Proof.
+  intros s. pose proof (m_isLe s) as H0.
+  simpl. destruct (m s) as [[x' s'] | ]; trivial.
+  simpl. pose proof (k_isLe x' s') as H1.
+  destruct (k x' s') as [[x'' s''] | ]; trivial. lia.
+Qed.
 
-  Example someP_example2
-    : (someP (satisfyP (fun ch : ascii => Ascii.eqb ch "a"%char)) (satisfyP_isLt _) "abc"%string)
-    = Some (["a"%char], "bc"%string).
-  Proof. reflexivity. Qed.
+Lemma pure_isLe {A : Type} (x : A)
+  : isLe (pure (A := A) x).
+Proof. intros s. simpl. reflexivity. Qed.
 
-  Example someP_example3
-    : (someP (satisfyP (fun ch : ascii => Ascii.eqb ch "b"%char)) (satisfyP_isLt _) "abc"%string)
-    = None.
-  Proof. reflexivity. Qed.
+Lemma alt_p1_p2_isLt_if_p1_isLt_and_p2_isLt {A : Type} (p1 : parser A) (p2 : parser A)
+  (p1_isLt : isLt p1)
+  (p2_isLt : isLt p2)
+  : isLt (alt (A := A) p1 p2).
+Proof.
+  intros s. simpl. pose proof (p1_isLt s) as H1. destruct (p1 s) as [[x s'] | ].
+  - eapply H1.
+  - pose proof (p2_isLt s) as H2. destruct (p2 s) as [[x' s'] | ]; trivial.
+Qed.
 
-  Lemma someP_unfold {A : Type} (p : parser A) (p_isLt : isLt p) (s : string) :
-    someP p p_isLt s =
-    match p s with
-    | None => None
-    | Some (x, s') =>
-      match someP p p_isLt s' with
-      | None => Some ([x], s')
-      | Some (xs, s'') => Some (x :: xs, s'')
-      end
-    end.
-  Proof.
-    unfold someP at 1; unfold someP_func; rewrite WfExtensionality.fix_sub_eq_ext; destruct (p s) as [[x s'] | ] eqn: OBS_p_s; simpl.
-    - rewrite OBS_p_s; destruct (someP p p_isLt s') as [[xs s''] | ] eqn: OBS_someP_p_s'.
-      + unfold someP, someP_func in OBS_someP_p_s'; rewrite OBS_someP_p_s'; reflexivity.
-      + unfold someP, someP_func in OBS_someP_p_s'; rewrite OBS_someP_p_s'; reflexivity.
-    - rewrite OBS_p_s; reflexivity.
-  Qed.
+Lemma alt_p1_p2_isLe_if_p1_isLe_and_p2_isLe {A : Type} (p1 : parser A) (p2 : parser A)
+  (p1_isLe : isLe p1)
+  (p2_isLe : isLe p2)
+  : isLe (alt (A := A) p1 p2).
+Proof.
+  intros s. simpl. pose proof (p1_isLe s) as H1. destruct (p1 s) as [[x s'] | ].
+  - eapply H1.
+  - pose proof (p2_isLe s) as H2. destruct (p2 s) as [[x' s'] | ]; trivial.
+Qed.
 
-  Lemma someP_isLt {A : Type} (p : parser A)
-    (p_isLt : isLt p)
-    : isLt (someP p p_isLt).
-  Proof.
-    intros s.
-    assert (H_Acc : Acc (fun s1 : string => fun s2 : string => length s1 < length s2) s) by exact (Prelude.acc_rel String.length lt Prelude.acc_lt s).
-    induction H_Acc as [s _ IH]. rewrite someP_unfold. pose proof (p_isLt s) as length_s_gt_length_s'. destruct (p s) as [[x s'] | ]; trivial. specialize (IH s' length_s_gt_length_s').
-    destruct (someP p p_isLt s') as [[xs s''] | ]; lia.
-  Qed.
+Lemma empty_isLt {A : Type}
+  : isLt (empty (A := A)).
+Proof.
+  intros s. simpl. trivial.
+Qed.
 
-  Definition manyP {A : Type} (p : parser A) (p_isLt : isLt p) : parser (list A) := someP p p_isLt <|> pure [].
+Section PARSER_COMBINATORS.
 
-  Theorem someP_spec {A : Type} (p : parser A) (p_isLt : isLt p)
-    : someP p p_isLt == (p >>= fun x => manyP p p_isLt >>= fun xs => pure (x :: xs)).
-  Proof. intros s. rewrite someP_unfold at 1. unfold manyP. simpl. destruct (p s) as [[x s'] | ]; try reflexivity. simpl. destruct (someP p p_isLt s') as [[xs s''] | ]; try reflexivity. Qed.
+Definition satisfyP (cond : char -> bool) : parser char :=
+  fun s : string =>
+  match s with
+  | []%string => None
+  | (ch :: s')%string => if cond ch then Some (ch, s') else None
+  end.
 
-  Theorem manyP_spec {A : Type} (p : parser A) (p_isLt : isLt p)
-    : manyP p p_isLt == someP p p_isLt <|> pure [].
-  Proof. reflexivity. Qed.
+Lemma satisfyP_isLt (cond : char -> bool)
+  : isLt (satisfyP cond).
+Proof.
+  intros s. unfold satisfyP. destruct s as [ | ch s']; trivial.
+  destruct (cond ch); trivial. simpl. red. reflexivity.
+Qed.
 
-  Lemma someP_lifts_eqP {A : Type} (p1 : parser A) (p1_isLt : isLt p1) (p2 : parser A) (p2_isLt : isLt p2)
-    (p1_eq_p2 : p1 == p2)
-    : someP p1 p1_isLt == someP p2 p2_isLt.
-  Proof.
-    intros s.
-    assert (H_Acc : Acc (fun s1 : string => fun s2 : string => length s1 < length s2) s) by exact (Prelude.acc_rel String.length lt Prelude.acc_lt s).
-    induction H_Acc as [s _ IH]. do 2 rewrite someP_unfold.
-    pose proof (p1_eq_p2 s) as p1_s_eq_p2_s. rewrite p1_s_eq_p2_s. destruct (p2 s) as [[x s'] | ]; trivial.
-    rewrite IH; trivial. pose proof (p1_isLt s) as length_s_gt_length_s'. rewrite p1_s_eq_p2_s in length_s_gt_length_s'. assumption.
-  Qed.
+Definition itemP : parser char :=
+  satisfyP (fun ch : char => true).
 
-  Lemma manyP_lifts_eqP {A : Type} (p1 : parser A) (p1_isLt : isLt p1) (p2 : parser A) (p2_isLt : isLt p2)
-    (p1_eq_p2 : p1 == p2)
-    : manyP p1 p1_isLt == manyP p2 p2_isLt.
-  Proof. now unfold manyP; rewrite someP_lifts_eqP with (p1_isLt := p1_isLt) (p2_isLt := p2_isLt) (p1_eq_p2 := p1_eq_p2). Qed.
+Lemma itemP_isLt
+  : isLt itemP.
+Proof. eapply satisfyP_isLt. Qed.
 
-  Definition spaceP : parser unit :=
-    (manyP (satisfyP (fun ch : ascii => Ascii.eqb ch " "%char)) (satisfyP_isLt _)) >>= fun _ => pure (isMonad := parserT_isMonad option_isMonad) tt.
+Definition stringP : string -> parser unit := sequenceM_ ∘ mapFromString (satisfyP ∘ Ascii.eqb).
 
-  Definition tokenP {A : Type} (p : parser A) : parser A :=
-    spaceP >>= fun _ => p >>= fun v => spaceP >>= fun _ => pure v.
+Lemma stringP_isLt (s : string)
+  (s_ne_nil : length s > 0)
+  : isLt (stringP s).
+Proof.
+  rename s into str, s_ne_nil into length_str_gt_0.
+  enough (to_show : length str = 0 \/ isLt (stringP str)).
+  { destruct to_show; [lia | eassumption]. }
+  clear length_str_gt_0. induction str as [ | ch str IH_str].
+  - left. reflexivity.
+  - simpl. right. intros s.
+    revert ch str IH_str. induction (string_wf s) as [s _ IH]. intros. simpl.
+    red. red. simpl. red. pose proof (satisfyP_isLt (Ascii.eqb ch) s) as length_s_gt_length_s'.
+    destruct (satisfyP (Ascii.eqb ch) s) as [[x s'] | ] eqn: H_OBS; trivial.
+    simpl. specialize (IH s' length_s_gt_length_s'). destruct str as [ | ch' str'].
+    + assert (IH_claim : length "" = 0 \/ isLt (stringP "")).
+      { left. reflexivity. }
+      specialize (IH ch []%string IH_claim). do 2 red in IH. simpl in IH. red in IH. simpl. eassumption.
+    + assert (IH_claim : length (ch' :: str')%string = 0 \/ isLt (stringP (ch' :: str')%string)).
+      { right. destruct IH_str as [IH_str | IH_str]; [inversion IH_str | eassumption]. }
+      specialize (IH ch (ch' :: str')%string IH_claim). do 2 red in IH. simpl in IH. red in IH.
+      destruct IH_str as [IH_str | IH_str].
+      * inversion IH_str.
+      * specialize (IH_str s'). red in IH_str. red in IH_str.
+        destruct (sequenceM_ (mapFromString (satisfyP ∘ Ascii.eqb) (ch' :: str')%string) s') as [[x' s''] | ] eqn: H_OBS'; trivial. lia.
+Qed.
 
-  Definition symbolP (s : string) : parser unit :=
-    tokenP (stringP s).
+Lemma stringP_isLe (s : string)
+  : isLe (stringP s).
+Proof.
+  destruct s as [ | ch s'].
+  - intros s. cbn. lia.
+  - eapply isLt_implies_isLe. eapply stringP_isLt. cbn. lia.
+Qed.
 
-  Let isNum (ch : ascii) : bool := Ascii.leb "0"%char ch && Ascii.leb ch "9"%char.
+#[program]
+Fixpoint someP {A : Type} (p : parser A) (p_isLt : isLt p) (s : string) {measure (length s)} : option (list A * string) :=
+  match p s with
+  | None => None
+  | Some (x, s') =>
+    match someP p p_isLt s' with
+    | None => Some ([x], s')
+    | Some (xs, s'') => Some (x :: xs, s'')
+    end
+  end.
+Next Obligation. pose proof (p_isLt s) as H. rewrite <- Heq_anonymous in H. eassumption. Defined.
 
-  Definition digitP : parser ascii := satisfyP isNum.
+Lemma someP_unfold {A : Type} (p : parser A) (p_isLt : isLt p) (s : string) :
+  someP p p_isLt s =
+  match p s with
+  | None => None
+  | Some (x, s') =>
+    match someP p p_isLt s' with
+    | None => Some ([x], s')
+    | Some (xs, s'') => Some (x :: xs, s'')
+    end
+  end.
+Proof.
+  unfold someP at 1; unfold someP_func; rewrite WfExtensionality.fix_sub_eq_ext; destruct (p s) as [[x s'] | ] eqn: OBS_p_s; simpl.
+  - rewrite OBS_p_s; destruct (someP p p_isLt s') as [[xs s''] | ] eqn: OBS_someP_p_s'.
+    + unfold someP, someP_func in OBS_someP_p_s'; rewrite OBS_someP_p_s'; reflexivity.
+    + unfold someP, someP_func in OBS_someP_p_s'; rewrite OBS_someP_p_s'; reflexivity.
+  - rewrite OBS_p_s; reflexivity.
+Qed.
 
-  Let isLower (ch : ascii) : bool := Ascii.leb "a"%char ch && Ascii.leb ch "z"%char.
+Lemma someP_isLt {A : Type} (p : parser A)
+  (p_isLt : isLt p)
+  : isLt (someP p p_isLt).
+Proof.
+  intros s. induction (string_wf s) as [s _ IH]. rewrite someP_unfold. pose proof (p_isLt s) as length_s_gt_length_s'. destruct (p s) as [[x s'] | ]; trivial. specialize (IH s' length_s_gt_length_s').
+  destruct (someP p p_isLt s') as [[xs s''] | ]; lia.
+Qed.
 
-  Definition lowerP : parser ascii := satisfyP isLower.
+Definition manyP {A : Type} (p : parser A) (p_isLt : isLt p) : parser (list A) := someP p p_isLt <|> pure [].
 
-  Let isUpper (ch : ascii) : bool := Ascii.leb "A"%char ch && Ascii.leb ch "Z"%char.
+Lemma manyP_isLe {A : Type} (p : parser A)
+  (p_isLt : isLt p)
+  : isLe (manyP p p_isLt).
+Proof.
+  intros s. unfold manyP. simpl.
+  pose proof (someP_isLt p p_isLt s) as H1.
+  destruct (someP p p_isLt s) as [[x s'] | ].
+  - lia.
+  - simpl. reflexivity.
+Qed.
 
-  Definition upperP : parser ascii := satisfyP isUpper.
+Theorem someP_defn {A : Type} (p : parser A) (p_isLt : isLt p)
+  : someP p p_isLt == (p >>= fun x => manyP p p_isLt >>= fun xs => pure (x :: xs)).
+Proof. intros s. rewrite someP_unfold at 1. unfold manyP. simpl. destruct (p s) as [[x s'] | ]; try reflexivity. simpl. destruct (someP p p_isLt s') as [[xs s''] | ]; try reflexivity. Qed.
 
-  Let isAlpha (ch : ascii) : bool := isLower ch || isUpper ch.
+Theorem manyP_defn {A : Type} (p : parser A) (p_isLt : isLt p)
+  : manyP p p_isLt == someP p p_isLt <|> pure [].
+Proof. reflexivity. Qed.
 
-  Definition letterP : parser ascii := satisfyP isAlpha.
+Lemma someP_lifts_eqP {A : Type} (p1 : parser A) (p1_isLt : isLt p1) (p2 : parser A) (p2_isLt : isLt p2)
+  (p1_eq_p2 : p1 == p2)
+  : someP p1 p1_isLt == someP p2 p2_isLt.
+Proof.
+  intros s. induction (string_wf s) as [s _ IH]. do 2 rewrite someP_unfold.
+  pose proof (p1_eq_p2 s) as p1_s_eq_p2_s. rewrite p1_s_eq_p2_s. destruct (p2 s) as [[x s'] | ]; trivial.
+  rewrite IH; trivial. pose proof (p1_isLt s) as length_s_gt_length_s'. rewrite p1_s_eq_p2_s in length_s_gt_length_s'. eassumption.
+Qed.
 
-  Let isAlphaNum (ch : ascii) : bool := isAlpha ch || isNum ch.
+Lemma manyP_lifts_eqP {A : Type} (p1 : parser A) (p1_isLt : isLt p1) (p2 : parser A) (p2_isLt : isLt p2)
+  (p1_eq_p2 : p1 == p2)
+  : manyP p1 p1_isLt == manyP p2 p2_isLt.
+Proof. now unfold manyP; rewrite someP_lifts_eqP with (p1_isLt := p1_isLt) (p2_isLt := p2_isLt) (p1_eq_p2 := p1_eq_p2). Qed.
 
-  Definition alphanumP : parser ascii := satisfyP isAlphaNum.
+Definition spaceP : parser unit :=
+  (manyP (satisfyP (fun ch : char => Ascii.eqb ch " "%char)) (satisfyP_isLt _)) >>= fun _ => pure tt.
 
-  Definition charP (ch : ascii) : parser unit := satisfyP (Ascii.eqb ch) >>= fun _ => pure tt.
+Lemma spaceP_isLe
+  : isLe spaceP.
+Proof.
+  eapply bind_m_k_isLe_if_m_isLe_and_k_isLe.
+  - eapply manyP_isLe.
+  - intros _. eapply pure_isLe.
+Qed.
 
-  Definition optMinusP : parser bool :=
-    (symbolP "-" >>= fun _ => pure true) <|> pure false.
+Definition tokenP {A : Type} (p : parser A) : parser A :=
+  spaceP >>= fun _ => p >>= fun v => spaceP >>= fun _ => pure v.
 
-  Definition naturalP : parser nat :=
-    (someP digitP (satisfyP_isLt (fun ch : ascii => ("0" <=? ch)%char && (ch <=? "9")%char))) >>= (fun s => pure (nat_from_string (mk_string s))).
+Lemma tokenP_isLt {A : Type} (p : parser A)
+  (p_isLt : isLt p)
+  : isLt (tokenP p).
+Proof.
+  unfold tokenP. eapply bind_m_k_isLt_if_m_isLe_and_k_isLt.
+  - eapply spaceP_isLe.
+  - intros _. eapply bind_m_k_isLt_if_m_isLt_and_k_isLe.
+    + exact (p_isLt).
+    + intros x. eapply bind_m_k_isLe_if_m_isLe_and_k_isLe.
+      * eapply spaceP_isLe.
+      * intros _. eapply pure_isLe.
+Qed.
 
-  Definition integerP : parser Z :=
-    optMinusP >>= fun b =>
-    naturalP >>= fun n =>
-    if b then pure ((-1) * Z.of_nat n)%Z else pure (Z.of_nat n).
+Lemma tokenP_isLe {A : Type} (p : parser A)
+  (p_isLe : isLe p)
+  : isLe (tokenP p).
+Proof.
+  unfold tokenP. eapply bind_m_k_isLe_if_m_isLe_and_k_isLe.
+  - eapply spaceP_isLe.
+  - intros _. eapply bind_m_k_isLe_if_m_isLe_and_k_isLe.
+    + exact (p_isLe).
+    + intros x. eapply bind_m_k_isLe_if_m_isLe_and_k_isLe.
+      * eapply spaceP_isLe.
+      * intros _. eapply pure_isLe.
+Qed.
 
-  Definition identP : parser string :=
-    lowerP >>= fun x => manyP alphanumP (satisfyP_isLt _) >>= fun xs => pure (String x (mk_string xs)).
+Definition symbolP (s : string) : parser unit :=
+  tokenP (stringP s).
 
-  Definition identifierP : parser string := tokenP identP.
+Lemma symbolP_isLt (s : string)
+  (s_ne_nil : length s > 0)
+  : isLt (symbolP s).
+Proof. eapply tokenP_isLt. eapply stringP_isLt. eassumption. Qed.
 
-  End PARSER_COMBINATORS.
+Definition digitP : parser char :=
+  satisfyP isNum.
+
+Lemma digitP_isLt
+  : isLt digitP.
+Proof. eapply satisfyP_isLt. Qed.
+
+Definition lowerP : parser char :=
+  satisfyP isLower.
+
+Lemma lowerP_isLt
+  : isLt lowerP.
+Proof. eapply satisfyP_isLt. Qed.
+
+Definition upperP : parser char :=
+  satisfyP isUpper.
+
+Lemma upperP_isLt
+  : isLt upperP.
+Proof. eapply satisfyP_isLt. Qed.
+
+Definition letterP : parser char :=
+  satisfyP isAlpha.
+
+Lemma letterP_isLt
+  : isLt letterP.
+Proof. eapply satisfyP_isLt. Qed.
+
+Definition alphanumP : parser char :=
+  satisfyP isAlphaNum.
+
+Lemma alphanumP_isLt
+  : isLt alphanumP.
+Proof. eapply satisfyP_isLt. Qed.
+
+Definition charP (ch : char) : parser unit :=
+  satisfyP (Ascii.eqb ch) >>= fun _ => pure tt.
+
+Lemma charP_isLt (ch : char)
+  : isLt (charP ch).
+Proof.
+  eapply bind_m_k_isLt_if_m_isLt_and_k_isLe.
+  - eapply satisfyP_isLt.
+  - intros _. eapply pure_isLe.
+Qed.
+
+Definition optMinusP : parser bool :=
+  (symbolP "-" >>= fun _ => pure true) <|> pure false.
+
+Lemma optMinusP_isLe
+  : isLe optMinusP.
+Proof.
+  eapply alt_p1_p2_isLe_if_p1_isLe_and_p2_isLe.
+  - eapply bind_m_k_isLe_if_m_isLe_and_k_isLe.
+    + eapply isLt_implies_isLe. eapply symbolP_isLt. simpl; eauto.
+    + intros _. eapply pure_isLe.
+  - eapply pure_isLe. 
+Qed.
+
+Definition naturalP : parser nat :=
+  (someP digitP (satisfyP_isLt (fun ch : char => ("0" <=? ch)%char && (ch <=? "9")%char))) >>= (fun s => pure (nat_from_string (mk_string s))).
+
+Lemma naturalP_isLt
+  : isLt naturalP.
+Proof.
+  eapply bind_m_k_isLt_if_m_isLt_and_k_isLe.
+  - eapply someP_isLt.
+  - intros str. eapply pure_isLe.
+Qed.
+
+Definition integerP : parser Z :=
+  optMinusP >>= fun b => naturalP >>= fun n => if b then pure ((-1) * Z.of_nat n)%Z else pure (Z.of_nat n).
+
+Lemma integerP_isLt
+  : isLt integerP.
+Proof.
+  eapply bind_m_k_isLt_if_m_isLe_and_k_isLt.
+  - eapply alt_p1_p2_isLe_if_p1_isLe_and_p2_isLe.
+    + eapply bind_m_k_isLe_if_m_isLe_and_k_isLe.
+      * eapply isLt_implies_isLe. eapply tokenP_isLt. eapply stringP_isLt. eauto.
+      * intros _. eapply pure_isLe.
+    + eapply pure_isLe.
+  - intros b. eapply bind_m_k_isLt_if_m_isLt_and_k_isLe.
+    + eapply naturalP_isLt.
+    + intros n. destruct b as [ | ].
+      * eapply pure_isLe.
+      * eapply pure_isLe.
+Qed.
+
+Definition identP : parser string :=
+  lowerP >>= fun x => manyP alphanumP (satisfyP_isLt _) >>= fun xs => pure (x :: mk_string xs)%string.
+
+Lemma identP_isLt
+  : isLt identP.
+Proof.
+  eapply bind_m_k_isLt_if_m_isLt_and_k_isLe.
+  - eapply satisfyP_isLt.
+  - intros ch. eapply bind_m_k_isLe_if_m_isLe_and_k_isLe.
+    + eapply manyP_isLe.
+    + intros chs. eapply pure_isLe.
+Qed.
+
+Definition identifierP : parser string :=
+  tokenP identP.
+
+Lemma identifierP_isLt
+  : isLt identifierP.
+Proof.
+  eapply tokenP_isLt. eapply identP_isLt.
+Qed.
+
+End PARSER_COMBINATORS.
 
 End P.
 
 Module Hs.
 
-  Import ListNotations.
+Import StringNotations ListNotations.
 
-  Inductive strSQLElem : Set :=
-  | Text : string -> strSQLElem
-  | Hole : string -> strSQLElem.
+Inductive strSQLElem : Set :=
+| Text : string -> strSQLElem
+| Hole : string -> strSQLElem.
 
-  Inductive value : Set :=
-  | ColName : string -> value
-  | StrVal  : string -> value
-  | IntVal  : Z      -> value
-  | Var     : string -> value.
+Inductive value : Set :=
+| ColName : string -> value
+| StrVal  : string -> value
+| IntVal  : Z      -> value
+| Var     : string -> value.
 
-  Inductive term : Set := 
-  | equalTerm : value -> value -> term.
+Inductive term : Set := 
+| equalTerm : value -> value -> term.
 
-  Inductive pred : Set := 
-  | orPred : pred -> pred -> pred
-  | termPred : term -> pred.
+Inductive pred : Set := 
+| orPred : pred -> pred -> pred
+| termPred : term -> pred.
 
-  Inductive cols : Set :=
-  | star : cols
-  | colNames : list string -> cols.
+Inductive cols : Set :=
+| star : cols
+| colNames : list string -> cols.
 
-  Inductive sql : Set :=
-  | sqlSFW : cols -> string -> option pred -> sql.
+Inductive sql : Set :=
+| sqlSFW : cols -> string -> option pred -> sql.
 
-  Fixpoint normPred_measure (p : pred) {struct p} : nat :=
-    match p with
-    | termPred t => 0
-    | orPred p1 p2 => 1 + (2 * normPred_measure p1 + normPred_measure p2)
-    end.
+#[global]
+Instance cols_hasEqDec
+  : hasEqDec cols.
+Proof with try ((left; congruence) || (right; congruence)).
+  change (forall lhs : cols, forall rhs : cols, {lhs = rhs} + {lhs <> rhs}).
+  intros [ | x] [ | y]...
+  pose proof (Prelude.eq_dec x y) as [H_EQ | H_NE]...
+Defined.
 
-  #[program]
-  Fixpoint normPred (p : pred) {measure (normPred_measure p)} : pred :=
-    match p with
-    | termPred t => termPred t
-    | orPred (termPred t1) p2 => orPred (termPred t1) (normPred p2)
-    | orPred (orPred p11 p12) p2 => normPred (orPred p11 (orPred p12 p2))
-    end.
-  Next Obligation. simpl. lia. Defined.
+#[global]
+Instance value_hasEqDec
+  : hasEqDec value.
+Proof with try ((left; congruence) || (right; congruence)).
+  change (forall lhs : value, forall rhs : value, {lhs = rhs} + {lhs <> rhs}).
+  induction lhs as [cn1 | s1 | i1 | v1], rhs as [cn2 | s2 | i2 | v2]...
+  - pose proof (Prelude.eq_dec cn1 cn2) as [H_EQ | H_NE]...
+  - pose proof (Prelude.eq_dec s1 s2) as [H_EQ | H_NE]...
+  - pose proof (Prelude.eq_dec i1 i2) as [H_EQ | H_NE]...
+  - pose proof (Prelude.eq_dec v1 v2) as [H_EQ | H_NE]...
+Defined.
 
-  Example normPred_example1
-    : (normPred (orPred (orPred (termPred (equalTerm (ColName "A") (ColName "B"))) (termPred (equalTerm (ColName "C") (ColName "D")))) (termPred (equalTerm (ColName "E") (ColName "F")))))
-    = orPred (termPred (equalTerm (ColName "A") (ColName "B"))) (orPred (termPred (equalTerm (ColName "C") (ColName "D"))) (termPred (equalTerm (ColName "E") (ColName "F")))).
-  Proof. reflexivity. Qed.
+#[global]
+Instance term_hasEqDec
+  : hasEqDec term.
+Proof with try ((left; congruence) || (right; congruence)).
+  change (forall lhs : term, forall rhs : term, {lhs = rhs} + {lhs <> rhs}).
+  intros [v1_1 v2_1] [v1_2 v2_2].
+  pose proof (Prelude.eq_dec v1_1 v1_2) as [H_EQ1 | H_NE1]...
+  pose proof (Prelude.eq_dec v2_1 v2_2) as [H_EQ2 | H_NE2]...
+Defined.
 
-  Lemma normPred_unfold (p : pred) :
-    normPred p =
-    match p with
-    | termPred t => termPred t
-    | orPred (termPred t1) p2 => orPred (termPred t1) (normPred p2)
-    | orPred (orPred p11 p12) p2 => normPred (orPred p11 (orPred p12 p2))
-    end.
-  Proof with eauto.
-    unfold normPred at 1. rewrite fix_sub_eq.
-    - destruct p as [[? ? | ?] | ?]...
-    - intros. destruct x as [[? ? | ?] | ?]; simpl... rewrite H...
-  Qed.
+#[global]
+Instance pred_hasEqDec
+  : hasEqDec pred.
+Proof with try ((left; congruence) || (right; congruence)).
+  change (forall lhs : pred, forall rhs : pred, {lhs = rhs} + {lhs <> rhs}).
+  induction lhs as [p1_1 IH1 p2_1 IH2 | t_1], rhs as [p1_2 p2_2 | t_2]...
+  - pose proof (IH1 p1_2) as [H_EQ1 | H_NE1]...
+    pose proof (IH2 p2_2) as [H_EQ2 | H_NE2]...
+  - pose proof (Prelude.eq_dec t_1 t_2) as [H_EQ | H_NE]... 
+Defined.
 
-  Definition normMaybePred (maybePred : option pred) : option pred :=
-    match maybePred with
+#[global]
+Instance sql_hasEqDec
+  : hasEqDec sql.
+Proof with try ((left; congruence) || (right; congruence)).
+  change (forall lhs : sql, forall rhs : sql, {lhs = rhs} + {lhs <> rhs}).
+  intros [x1 x2 [x3 | ]] [y1 y2 [y3 | ]]...
+  - pose proof (Prelude.eq_dec x1 y1) as [H_EQ1 | H_NE1]...
+    pose proof (Prelude.eq_dec x2 y2) as [H_EQ2 | H_NE2]...
+    pose proof (Prelude.eq_dec x3 y3) as [H_EQ3 | H_NE3]...
+  - pose proof (Prelude.eq_dec x1 y1) as [H_EQ1 | H_NE1]...
+    pose proof (Prelude.eq_dec x2 y2) as [H_EQ2 | H_NE2]...
+Defined.
+
+Section NORM.
+
+Fixpoint normPred_measure (p : pred) {struct p} : nat :=
+  match p with
+  | termPred t => 0
+  | orPred p1 p2 => 1 + (2 * normPred_measure p1 + normPred_measure p2)
+  end.
+
+#[program]
+Fixpoint normPred (p : pred) {measure (normPred_measure p)} : pred :=
+  match p with
+  | termPred t => termPred t
+  | orPred (termPred t1) p2 => orPred (termPred t1) (normPred p2)
+  | orPred (orPred p11 p12) p2 => normPred (orPred p11 (orPred p12 p2))
+  end.
+Next Obligation.
+  simpl. repeat rewrite Nat.add_0_r; red. lia.
+Defined.
+
+Example normPred_example1
+  (p1 := termPred (equalTerm (ColName "A") (ColName "B")))
+  (p2 := termPred (equalTerm (ColName "D") (ColName "E")))
+  (p3 := termPred (equalTerm (ColName "G") (ColName "H")))
+  (p4 := termPred (equalTerm (ColName "J") (ColName "K")))
+  : normPred (orPred (orPred p1 p2) (orPred p3 p4))
+  = orPred p1 (orPred p2 (orPred p3 p4)).
+Proof. reflexivity. Qed.
+
+Lemma normPred_unfold (p : pred) :
+  normPred p =
+  match p with
+  | termPred t => termPred t
+  | orPred (termPred t1) p2 => orPred (termPred t1) (normPred p2)
+  | orPred (orPred p11 p12) p2 => normPred (orPred p11 (orPred p12 p2))
+  end.
+Proof with eauto.
+  unfold normPred at 1. rewrite fix_sub_eq.
+  - destruct p as [[? ? | ?] | ?]...
+  - intros. destruct x as [[? ? | ?] | ?]; simpl... rewrite H...
+Qed.
+
+Definition normMaybePred (maybePred : option pred) : option pred :=
+  match maybePred with
+  | None => None
+  | Some pred => Some (normPred pred)
+  end.
+
+Definition norm (sql : Hs.sql) : Hs.sql :=
+  match sql with
+  | sqlSFW cols tbl maybePred => sqlSFW cols tbl (normMaybePred maybePred)
+  end.
+
+End NORM.
+
+Definition env : Set := list (string * value).
+
+Section APPLY.
+
+Definition applyValue (e : env) (v : value) : value :=
+  match v with
+  | ColName cn => ColName cn
+  | StrVal s => StrVal s
+  | IntVal i => IntVal i
+  | Var x =>
+    match lookup x e with
+    | None => Var x
+    | Some v' => v'
+    end
+  end.
+
+Definition applyTerm (e : env) (t : term) : term :=
+  match t with
+  | equalTerm v1 v2 => equalTerm (applyValue e v1) (applyValue e v2)
+  end.
+
+Fixpoint applyPred (e : env) (p : pred) : pred :=
+  match p with
+  | termPred t => termPred (applyTerm e t)
+  | orPred p1 p2 => orPred (applyPred e p1) (applyPred e p2)
+  end.
+
+Definition applyMaybePred (e : env) (maybePred : option pred) : option pred :=
+  match maybePred with
+  | None => None
+  | Some p => Some (applyPred e p)
+  end.
+
+Definition applySQL (e : env) (sql : Hs.sql) : Hs.sql :=
+  match sql with
+  | sqlSFW cols tbl maybePred => sqlSFW cols tbl (applyMaybePred e maybePred)
+  end.
+
+End APPLY.
+
+Definition injection (v : string) (s : string) (sql : Hs.sql) : Hs.sql := applySQL [(v, StrVal s)] sql.
+
+Section INJECTION_FREE.
+
+Definition injFreeValue (lhs : value) (rhs : value) : bool :=
+  match lhs, rhs with
+  | ColName c1, ColName c2 => Prelude.eqb c1 c2
+  | StrVal s1, StrVal s2 => Prelude.eqb s1 s2
+  | IntVal i1, IntVal i2 => Prelude.eqb i1 i2
+  | Var x, _ => true
+  | _, Var x => true
+  | _, _ => false
+  end.
+
+Definition injFreeTerm (lhs : term) (rhs : term) : bool :=
+  match lhs, rhs with
+  | equalTerm v11 v12, equalTerm v21 v22 => injFreeValue v11 v21 && injFreeValue v12 v22
+  end.
+
+Fixpoint injFreePred (lhs : pred) (rhs : pred) : bool :=
+  match lhs, rhs with
+  | termPred t1, termPred t2 => injFreeTerm t1 t2
+  | orPred pred11 pred12, orPred pred21 pred22 => injFreePred pred11 pred21 && injFreePred pred12 pred22
+  | _, _ => false
+  end.
+
+Definition injFreeMaybePred (lhs : option pred) (rhs : option pred) : bool :=
+  match lhs, rhs with
+  | Some p1, Some p2 => injFreePred p1 p2
+  | None, None => true
+  | _, _ => false
+  end.
+
+Definition injFree (s1 : sql) (s2 : sql) : bool :=
+  match s1, s2 with
+  | sqlSFW cols1 tbl1 maybePred1, sqlSFW cols2 tbl2 maybePred2 => Prelude.eqb cols1 cols2 && Prelude.eqb tbl1 tbl2 && injFreeMaybePred maybePred1 maybePred2
+  end.
+
+End INJECTION_FREE.
+
+Section PRINTER.
+
+Fixpoint ppString1 (s : string) : string :=
+  match s with
+  | []%string => ""%string
+  | ("'"%char :: s')%string => ("''" ++ ppString1 s')%string
+  | (ch :: s')%string => (ch :: ppString1 s')%string
+  end.
+
+Definition ppString (s : string) : string :=
+  String_concat ["'"%string; ppString1 s; "'"%string]%list.
+
+Definition ppValue (v : value) : string :=
+  match v with
+  | ColName s => s
+  | StrVal s => ppString s
+  | IntVal i => Z_to_string i
+  | Var x => ("{" ++ x ++ "}")%string
+  end.
+
+Definition ppTerm (t : term) : string :=
+  match t with
+  | equalTerm v1 v2 => String_concat [ppValue v1; " = "%string; ppValue v2]
+  end.
+
+Fixpoint ppPred (p : pred) : string :=
+  match p with
+  | termPred t => ppTerm t
+  | orPred p q => String_concat [ppPred p; " or "%string; ppPred q]
+  end.
+
+Definition ppWhere (maybePred : option pred) : string :=
+  match maybePred with
+  | None => ""%string
+  | Some pred => String_concat [" where "%string; ppPred pred]
+  end.
+
+Definition ppTbl (tbl : string) : string := tbl.
+
+Fixpoint ppCols_aux (cs : list string) {struct cs} : string :=
+  match cs with
+  | [] => ""%string
+  | [c1] => c1
+  | c1 :: cs' => String_concat [c1; ","%string; ppCols_aux cs']
+  end.
+
+Definition ppCols (c : cols) : string :=
+  match c with
+  | star => "*"%string
+  | colNames cs => ppCols_aux cs
+  end.
+
+Definition printSQL (s : sql) : string :=
+  match s with
+  | sqlSFW cols tbl maybePred => String_concat ["select "%string; ppCols cols; " from "%string; ppTbl tbl; ppWhere maybePred]
+  end.
+
+End PRINTER.
+
+Section PARSER.
+
+#[program]
+Fixpoint sqlstringinP (s0 : string) {measure (length s0)} : option (string * string) :=
+  match
+    match P.charP "'"%char s0 with
     | None => None
-    | Some pred => Some (normPred pred)
-    end.
-
-  Definition norm (s : sql) : sql :=
-    match s with
-    | sqlSFW cols tbl maybePred => sqlSFW cols tbl (normMaybePred maybePred)
-    end.
-
-  Definition env : Set := list (string * value).
-
-  Definition applyValue (e : env) (v : value) : value :=
-    match v with
-    | ColName cn => ColName cn
-    | StrVal s => StrVal s
-    | IntVal i => IntVal i
-    | Var x =>
-      match lookup x (string_dec x) e with
-      | None => Var x
-      | Some v' => v'
+    | Some (_, s1) =>
+      match P.charP "'"%char s1 with
+      | None => None
+      | Some (_, s2) =>
+        match sqlstringinP s2 with
+        | None => None
+        | Some (text, s3) => Some (("'"%char :: text)%string, s3)
+        end
       end
-    end.
+    end
+  with
+  | None =>
+    match
+      match P.charP "'"%char s0 with
+      | None => None
+      | Some (_, s1) => Some (""%string, s1)
+      end
+    with
+    | None =>
+      match P.itemP s0 with
+      | None => None
+      | Some (c, s1) =>
+        match sqlstringinP s1 with
+        | None => None
+        | Some (text, s2) => Some ((c :: text)%string, s2)
+        end
+      end
+    | Some res => Some res
+    end
+  | Some res => Some res
+  end.
+Next Obligation.
+  pose proof (P.charP_isLt "'"%char s1) as H1. rewrite <- Heq_anonymous in H1.
+  pose proof (P.charP_isLt "'"%char s0) as H2. rewrite <- Heq_anonymous0 in H2.
+  etransitivity; eassumption.
+Defined.
+Next Obligation.
+  pose proof (P.itemP_isLt s0) as H1. rewrite <- Heq_anonymous in H1.
+  eassumption.
+Defined.
 
-  Definition applyTerm (e : env) (t : term) : term :=
-    match t with
-    | equalTerm v1 v2 => equalTerm (applyValue e v1) (applyValue e v2)
-    end.
-
-  Fixpoint applyPred (e : env) (p : pred) : pred :=
-    match p with
-    | termPred t => termPred (applyTerm e t)
-    | orPred p1 p2 => orPred (applyPred e p1) (applyPred e p2)
-    end.
-
-  Definition applyMaybePred (e : env) (maybePred : option pred) : option pred :=
-    match maybePred with
+Lemma sqlstringinP_unfold (s0 : string) :
+  sqlstringinP s0 =
+  match
+    match P.charP "'"%char s0 with
     | None => None
-    | Some p => Some (applyPred e p)
-    end.
-
-  Definition applySQL (e : env) (s : sql) : sql :=
-    match s with
-    | sqlSFW cols tbl maybePred => sqlSFW cols tbl (applyMaybePred e maybePred)
-    end.
-
-  Definition injection (v : string) (s : string) : sql -> sql := applySQL [(v, StrVal s)].
-
-  Section INJECTION_FREE.
-
-  Lemma cols_eq_dec
-    : forall lhs : cols, forall rhs : cols, {lhs = rhs} + {lhs <> rhs}.
-    Proof with try ((left; congruence) || (right; congruence)).
-    intros [ | x] [ | y]...
-    pose proof (list_eq_dec string_dec x y) as [H_EQ | H_NE]...
-  Defined.
-
-  Lemma value_eq_dec
-    : forall lhs : value, forall rhs : value, {lhs = rhs} + {lhs <> rhs}.
-  Proof with try ((left; congruence) || (right; congruence)).
-    induction lhs as [cn1 | s1 | i1 | v1], rhs as [cn2 | s2 | i2 | v2]...
-    - pose proof (string_dec cn1 cn2) as [H_EQ | H_NE]...
-    - pose proof (string_dec s1 s2) as [H_EQ | H_NE]...
-    - pose proof (Z.eq_dec i1 i2) as [H_EQ | H_NE]...
-    - pose proof (string_dec v1 v2) as [H_EQ | H_NE]...
-  Defined.
-
-  Lemma term_eq_dec
-    : forall lhs : term, forall rhs : term, {lhs = rhs} + {lhs <> rhs}.
-  Proof with try ((left; congruence) || (right; congruence)).
-    intros [v1_1 v2_1] [v1_2 v2_2].
-    pose proof (value_eq_dec v1_1 v1_2) as [H_EQ1 | H_NE1]; pose proof (value_eq_dec v2_1 v2_2) as [H_EQ2 | H_NE2]...
-  Defined.
-
-  Lemma pred_eq_dec
-    : forall lhs : pred, forall rhs : pred, {lhs = rhs} + {lhs <> rhs}.
-  Proof with try ((left; congruence) || (right; congruence)).
-    induction lhs as [p1_1 IH1 p2_1 IH2 | t_1], rhs as [p1_2 p2_2 | t_2]...
-    - pose proof (IH1 p1_2) as [H_EQ1 | H_NE1]; pose proof (IH2 p2_2) as [H_EQ2 | H_NE2]...
-    - pose proof (term_eq_dec t_1 t_2) as [H_EQ | H_NE]... 
-  Defined.
-
-  Lemma sql_eq_dec
-    : forall lhs : sql, forall rhs : sql, {lhs = rhs} + {lhs <> rhs}.
-  Proof with try ((left; congruence) || (right; congruence)).
-    intros [x1 x2 [x3 | ]] [y1 y2 [y3 | ]]...
-    - pose proof (cols_eq_dec x1 y1) as [H_EQ1 | H_NE1]...
-      pose proof (string_dec x2 y2) as [H_EQ2 | H_NE2]...
-      pose proof (pred_eq_dec x3 y3) as [H_EQ3 | H_NE3]...
-    - pose proof (cols_eq_dec x1 y1) as [H_EQ1 | H_NE1]...
-      pose proof (string_dec x2 y2) as [H_EQ2 | H_NE2]...
-  Defined.
-
-  Definition injFreeValue (lhs : value) (rhs : value) : bool :=
-    match lhs, rhs with
-    | ColName c1, ColName c2 => eq_dec_to_bool string_dec c1 c2
-    | StrVal s1, StrVal s2 => eq_dec_to_bool string_dec s1 s2
-    | IntVal i1, IntVal i2 => eq_dec_to_bool Z.eq_dec i1 i2
-    | Var x, _ => true
-    | _, Var x => true
-    | _, _ => false
-    end.
-
-  Definition injFreeTerm (lhs : term) (rhs : term) : bool :=
-    match lhs, rhs with
-    | equalTerm v11 v12, equalTerm v21 v22 => injFreeValue v11 v21 && injFreeValue v12 v22
-    end.
-
-  Fixpoint injFreePred (lhs : pred) (rhs : pred) : bool :=
-    match lhs, rhs with
-    | termPred t1, termPred t2 => injFreeTerm t1 t2
-    | orPred pred11 pred12, orPred pred21 pred22 => injFreePred pred11 pred21 && injFreePred pred12 pred22
-    | _, _ => false
-    end.
-
-  Definition injFreeMaybePred (lhs : option pred) (rhs : option pred) : bool :=
-    match lhs, rhs with
-    | Some p1, Some p2 => injFreePred p1 p2
-    | None, None => true
-    | _, _ => false
-    end.
-
-  Definition injFree (s1 : sql) (s2 : sql) : bool :=
-    match s1, s2 with
-    | sqlSFW cols1 tbl1 maybePred1, sqlSFW cols2 tbl2 maybePred2 => eq_dec_to_bool cols_eq_dec cols1 cols2 && eq_dec_to_bool string_dec tbl1 tbl2 && injFreeMaybePred maybePred1 maybePred2
-    end.
-
-  End INJECTION_FREE.
-
-  Section PRINTER.
-
-  Fixpoint ppString1 (s : string) : string :=
-    match s with
-    | EmptyString => ""%string
-    | String "'"%char s' => ("''" ++ ppString1 s')%string
-    | String ch s' => String ch (ppString1 s')
-    end.
-
-  Definition ppString (s : string) : string :=
-    String_concat ["'"%string; ppString1 s; "'"%string]%list.
-
-  Definition ppValue (v : value) : string :=
-    match v with
-    | ColName s => s
-    | StrVal s => ppString s
-    | IntVal i => Z_to_string i
-    | Var x => ("{" ++ x ++ "}")%string
-    end.
-
-  Definition ppTerm (t : term) : string :=
-    match t with
-    | equalTerm v1 v2 => String_concat [ppValue v1; " = "%string; ppValue v2]
-    end.
-
-  Fixpoint ppPred (p : pred) : string :=
-    match p with
-    | termPred t => ppTerm t
-    | orPred p q => String_concat [ppPred p; " or "%string; ppPred q]
-    end.
-
-  Definition ppWhere (maybePred : option pred) : string :=
-    match maybePred with
-    | None => ""%string
-    | Some pred => String_concat [" where "%string; ppPred pred]
-    end.
-
-  Definition ppTbl (tbl : string) : string := tbl.
-
-  Definition ppCols (c : cols) : string :=
-    let go : list string -> string :=
-      fix go_fix (ss : list string) {struct ss} : string :=
-      match ss with
-      | [] => ""%string
-      | [c1] => c1
-      | c1 :: cs => String_concat [c1; ","%string; go_fix cs]
+    | Some (_, s1) =>
+      match P.charP "'"%char s1 with
+      | None => None
+      | Some (_, s2) =>
+        match sqlstringinP s2 with
+        | None => None
+        | Some (text, s3) => Some (("'"%char :: text)%string, s3)
+        end
       end
-    in
-    match c with
-    | star => "*"%string
-    | colNames cs => go cs
-    end.
+    end
+  with
+  | None =>
+    match
+      match P.charP "'"%char s0 with
+      | None => None
+      | Some (_, s1) => Some (""%string, s1)
+      end
+    with
+    | None =>
+      match P.itemP s0 with
+      | None => None
+      | Some (c, s1) =>
+        match sqlstringinP s1 with
+        | None => None
+        | Some (text, s2) => Some (("'"%char :: text)%string, s2)
+        end
+      end
+    | Some res => Some res
+    end
+  | Some res => Some res
+  end.
+Proof.
+Admitted.
 
-  Definition printSQL (s : sql) : string :=
-    match s with
-    | sqlSFW cols tbl maybePred => String_concat ["select "%string; ppCols cols; " from "%string; ppTbl tbl; ppWhere maybePred]
-    end.
+Theorem sqlstringinP_defn
+  : sqlstringinP == (P.charP "'"%char >>= fun _ => P.charP "'"%char >>= fun _ => sqlstringinP >>= fun text => pure (("'"%char :: text)%string)) <|> (P.charP "'"%char >>= fun _ => pure ""%string) <|> (P.itemP >>= fun c => sqlstringinP >>= fun text => pure ("'"%char :: text)%string).
+Proof with trivial.
+  intros s0. rewrite sqlstringinP_unfold at 1. simpl...
+  destruct (P.charP "'" s0) as [[x1 s1] | ] eqn: H_OBS1; simpl...
+  destruct (P.charP "'" s1) as [[x2 s2] | ] eqn: H_OBS2; simpl...
+  destruct (sqlstringinP s2) as [[x3 s3] | ] eqn: H_OBS3; simpl...
+Qed.
 
-  End PRINTER.
+Lemma sqlstringinP_isLt
+  : P.isLt sqlstringinP.
+Proof with trivial.
+  intros s. induction (P.string_wf s) as [s0 _ IH]. rewrite sqlstringinP_unfold; simpl.
+  pose proof (P.charP_isLt "'" s0) as H1. destruct (P.charP "'" s0) as [[x1 s1] | ] eqn: H_OBS1; simpl...
+  - pose proof (P.charP_isLt "'" s1) as H2. destruct (P.charP "'" s1) as [[x2 s2] | ] eqn: H_OBS2; simpl...
+    assert (length_gt : length s2 < length s0) by lia.
+    specialize (IH s2 length_gt). destruct (sqlstringinP s2) as [[x3 s3] | ] eqn: H_OBS3; simpl... lia.
+  - pose proof (P.itemP_isLt s0) as H2. destruct (P.itemP s0) as [[x1 s1] | ] eqn: H_OBS2...
+    specialize (IH s1 H2). destruct (sqlstringinP s1) as [[x3 s3] | ] eqn: H_OBS3... lia.
+Qed.
 
-  Section PARSER.
+Definition sqlstringP : P.parser string :=
+  P.charP "'"%char >>= fun _ => sqlstringinP >>= fun text => pure text.
 
-  Definition hacking {A : Type} (p_n : nat -> P.parser A) : P.parser A :=
-    fun s : string => p_n (length s) s.
+Lemma sqlstringP_isLt
+  : P.isLt sqlstringP.
+Proof.
+  eapply P.bind_m_k_isLt_if_m_isLt_and_k_isLe.
+  - eapply P.charP_isLt.
+  - intros _. eapply P.bind_m_k_isLe_if_m_isLe_and_k_isLe.
+    + eapply P.isLt_implies_isLe. eapply sqlstringinP_isLt.
+    + intros x. eapply P.pure_isLe.
+Qed.
 
-  Fixpoint sqlstringin' (n : nat) {struct n} : P.parser string :=
-    match n with
-    | O => pure ""%string
-    | S n' => (P.charP "'"%char >>= fun _ => P.charP "'"%char >>= fun _ => sqlstringin' n' >>= fun text => pure (String "'"%char text)) <|> (P.charP "'"%char >>= fun _ => pure ""%string) <|> (P.satisfyP (fun ch : ascii => true) >>= fun c : ascii => sqlstringin' n' >>= fun text => pure (String c text)) 
-    end.
+Definition parsevalueP : P.parser value :=
+  (P.identifierP >>= fun colName => pure (ColName colName)) <|> (sqlstringP >>= fun sqlstr => pure (StrVal sqlstr)) <|> (P.integerP >>= fun i => pure (IntVal i)) <|> (P.symbolP "{" >>= fun _ => P.identifierP >>= fun v => P.symbolP "}" >>= fun _ => pure (Var v)).
 
-  Definition sqlstringin : P.parser string := hacking sqlstringin'.
+Lemma parsevalueP_isLt
+  : P.isLt parsevalueP.
+Proof.
+  eapply P.alt_p1_p2_isLt_if_p1_isLt_and_p2_isLt.
+  - eapply P.alt_p1_p2_isLt_if_p1_isLt_and_p2_isLt.
+    + eapply P.alt_p1_p2_isLt_if_p1_isLt_and_p2_isLt.
+      * eapply P.bind_m_k_isLt_if_m_isLt_and_k_isLe.
+        { eapply P.tokenP_isLt. eapply P.identP_isLt. }
+        { intros s. eapply P.pure_isLe. }
+      * eapply P.bind_m_k_isLt_if_m_isLt_and_k_isLe.
+        { eapply sqlstringP_isLt. }
+        { intros s. eapply P.pure_isLe. }
+    + eapply P.bind_m_k_isLt_if_m_isLt_and_k_isLe.
+      * eapply P.integerP_isLt.
+      * intros i. eapply P.pure_isLe.
+  - eapply P.bind_m_k_isLt_if_m_isLt_and_k_isLe.
+    + eapply P.tokenP_isLt. eapply P.stringP_isLt. eauto.
+    + intros _. eapply P.bind_m_k_isLe_if_m_isLe_and_k_isLe.
+      * eapply P.isLt_implies_isLe. eapply P.identifierP_isLt.
+      * intros s. eapply P.isLt_implies_isLe. eapply P.bind_m_k_isLt_if_m_isLt_and_k_isLe.
+        { eapply P.tokenP_isLt. eapply P.stringP_isLt. eauto. }
+        { intros _. eapply P.pure_isLe. }
+Qed.
 
-  Definition sqlstring : P.parser string :=
-    P.charP "'"%char >>= fun _ => sqlstringin >>= fun text => pure text.
+Definition parsetermP : P.parser term :=
+  parsevalueP >>= fun v1 => P.symbolP "=" >>= fun _ => parsevalueP >>= fun v2 => pure (equalTerm v1 v2).
 
-  Definition parsevalue : P.parser value :=
-    (P.identifierP >>= fun colName => pure (ColName colName)) <|> (sqlstring >>= fun sqlstr => pure (StrVal sqlstr)) <|> (P.integerP >>= fun i => pure (IntVal i)) <|> (P.symbolP "{" >>= fun _ => P.identifierP >>= fun v => P.symbolP "}" >>= fun _ => pure (Var v)).
+Lemma parsetermP_isLt
+  : P.isLt parsetermP.
+Proof.
+  eapply P.bind_m_k_isLt_if_m_isLe_and_k_isLt.
+  - eapply P.isLt_implies_isLe. eapply parsevalueP_isLt.
+  - intros v. eapply P.bind_m_k_isLt_if_m_isLt_and_k_isLe.
+    + eapply P.tokenP_isLt. eapply P.stringP_isLt. eauto.
+    + intros _. eapply P.bind_m_k_isLe_if_m_isLe_and_k_isLe.
+      * eapply P.isLt_implies_isLe. eapply parsevalueP_isLt.
+      * intros v'. eapply P.pure_isLe.
+Qed.
 
-  Definition parseterm : P.parser term :=
-    parsevalue >>= fun v1 => P.symbolP "=" >>= fun _ => parsevalue >>= fun v2 => pure (equalTerm v1 v2).
+#[program]
+Fixpoint predicate1P (s0 : string) {measure (length s0)} : option ((pred -> pred) * string) :=
+  match
+    match P.symbolP "or"%string s0 with
+    | None => None
+    | Some (_, s1) =>
+      match
+        match parsetermP s1 with
+        | None => None
+        | Some (term, s2) =>
+          match predicate1P s2 with
+          | None => None
+          | Some (f, s3) => Some (f (termPred term), s3)
+          end
+        end
+      with
+      | None => None
+      | Some (pred2, s2) =>
+        match predicate1P s2 with
+        | None => None
+        | Some (f, s3) => Some ((fun pred1 => f (orPred pred1 pred2)), s3)
+        end
+      end
+    end
+  with
+  | None => Some ((fun x => x), s0)
+  | Some res => Some res
+  end.
+Next Obligation.
+  assert (claim : P.isLt (P.symbolP "or"%string)).
+  { eapply P.tokenP_isLt. eapply P.stringP_isLt. simpl. eauto. }
+  pose proof (claim s0) as H1. rewrite <- Heq_anonymous0 in H1. 
+  pose proof (parsetermP_isLt s1) as H2. rewrite <- Heq_anonymous in H2. lia.
+Defined.
+Next Obligation.
+Admitted.
 
-  Fixpoint predicate1' (n : nat) : P.parser (pred -> pred) :=
-    match n with
-    | O => pure (fun x => x)
-    | S n' => (P.symbolP "or" >>= fun _ => (parseterm >>= fun term => predicate1' n' >>= fun f => pure (f (termPred term))) >>= fun pred2 => predicate1' n' >>= fun f => pure (fun pred1 => f (orPred pred1 pred2))) <|> pure (fun x => x)
-    end.
+Lemma predicate1P_unfold (s0 : string) :
+  predicate1P s0 =
+  match
+    match P.symbolP "or"%string s0 with
+    | None => None
+    | Some (_, s1) =>
+      match
+        match parsetermP s1 with
+        | None => None
+        | Some (term, s2) =>
+          match predicate1P s2 with
+          | None => None
+          | Some (f, s3) => Some (f (termPred term), s3)
+          end
+        end
+      with
+      | None => None
+      | Some (pred2, s2) =>
+        match predicate1P s2 with
+        | None => None
+        | Some (f, s3) => Some ((fun pred1 => f (orPred pred1 pred2)), s3)
+        end
+      end
+    end
+  with
+  | None => Some ((fun x => x), s0)
+  | Some res => Some res
+  end.
+Proof.
+Admitted.
 
-  Definition predicate1 : P.parser (pred -> pred) := hacking predicate1'.
+Definition predicateP : P.parser pred :=
+  parsetermP >>= fun term => predicate1P >>= fun f => pure (f (termPred term)).
 
-  Definition predicate : P.parser pred :=
-    parseterm >>= fun term => predicate1 >>= fun f => pure (f (termPred term)).
+Theorem predicateP_defn
+  : predicateP == (parsetermP >>= fun term => predicate1P >>= fun f => pure (f (termPred term))).
+Proof. reflexivity. Qed.
 
-  Definition optWhere : P.parser (option pred) :=
-    (P.symbolP "where" >>= fun _ => predicate >>= fun pred => pure (Some pred)) <|> pure None.
+Theorem predicate1P_defn
+  : predicate1P == (P.symbolP "or" >>= fun _ => predicateP >>= fun pred2 => predicate1P >>= fun f => pure (fun pred1 => f (orPred pred1 pred2))) <|> pure (fun x => x).
+Proof with reflexivity || trivial.
+  transitivity ((P.symbolP "or" >>= (fun _ => (parsetermP >>= fun term => predicate1P >>= fun f => pure (f (termPred term))) >>= (fun pred2 => predicate1P >>= (fun f => pure (fun pred1 => f (orPred pred1 pred2)))))) <|> pure (fun x => x))...
+  intros s0. rewrite predicate1P_unfold at 1. simpl...
+Qed.
 
-  Definition table : P.parser string := P.identifierP.
+Definition optWhereP : P.parser (option pred) :=
+  (P.symbolP "where" >>= fun _ => predicateP >>= fun pred => pure (Some pred)) <|> pure None.
 
-  Axiom sorry1 : P.isLt (P.symbolP "," >>= (fun _ : () => P.identifierP)).
+Definition tableP : P.parser string := P.identifierP.
 
-  Definition columns1 : P.parser (list string) :=
-    P.identifierP >>= fun col => P.manyP (P.symbolP "," >>= fun _ => P.identifierP) sorry1 >>= fun cols => pure (col :: cols).
+#[program]
+Definition columns1P : P.parser (list string) :=
+  P.identifierP >>= fun col => P.manyP (P.symbolP "," >>= fun _ => P.identifierP) _ >>= fun cols => pure (col :: cols).
+Next Obligation.
+  change (P.isLt (P.symbolP "," >>= fun _ => P.identifierP)).
+  eapply P.bind_m_k_isLt_if_m_isLt_and_k_isLe.
+  - eapply P.symbolP_isLt. simpl; eauto.
+  - intros _. eapply P.isLt_implies_isLe. eapply P.identifierP_isLt. 
+Defined.
 
-  Definition columns : P.parser cols :=
-    columns1 >>= fun cols => pure (colNames cols).
+Definition columnsP : P.parser cols :=
+  columns1P >>= fun cols => pure (colNames cols).
 
-  Definition parseSQL : P.parser sql :=
-    P.symbolP "select" >>= fun _ => (P.symbolP "*" >>= fun _ => pure star) <|> columns >>= fun cols => P.symbolP "from" >>= fun _ => table >>= fun tbl => optWhere >>= fun maybePred => pure (sqlSFW cols tbl maybePred).
+Definition parseSQL : P.parser sql :=
+  P.symbolP "select" >>= fun _ => (P.symbolP "*" >>= fun _ => pure star) <|> columnsP >>= fun cols => P.symbolP "from" >>= fun _ => tableP >>= fun tbl => optWhereP >>= fun maybePred => pure (sqlSFW cols tbl maybePred).
 
-  End PARSER.
+End PARSER.
 
 End Hs.
 
 Module Main.
 
-  Import ListNotations.
+Import ListNotations.
 
-  Definition defaultSQL : Hs.sql :=
-    Hs.sqlSFW (Hs.colNames []) "" None.
+Definition must_return_true (sql : Hs.sql) (x : string) (v : string) : bool :=
+  match Hs.parseSQL ∘ Hs.printSQL ∘ Hs.injection x v $ sql with
+  | Some (sql', EmptyString) => Hs.injFree (Hs.norm sql) (Hs.norm sql')
+  | _ => false
+  end.
 
-  Definition sqlFrom (res : option (Hs.sql * string)) : Hs.sql :=
-    match res with
-    | Some (sql, ""%string) => sql
-    | _ => defaultSQL
-    end.
+Section SQL_EXAMPLES.
 
-  Definition spec (sql : Hs.sql) (x : string) (v : string) : bool :=
-    Hs.injFree (Hs.norm sql) ∘ Hs.norm ∘ sqlFrom ∘ Hs.parseSQL ∘ Hs.printSQL ∘ Hs.injection x v $ sql.
+Definition sql01 : Hs.sql :=
+  Hs.sqlSFW Hs.star "t"%string None.
 
-  Definition sql04 : Hs.sql :=
-    Hs.sqlSFW Hs.star "t" (Some (Hs.termPred (Hs.equalTerm (Hs.ColName "id") (Hs.IntVal 123)))).
+Example sql01_example1
+  (sql := sql01)
+  (x := "z"%string)
+  (v := "' or 1=1"%string)
+  : must_return_true sql x v
+  = true.
+Proof. reflexivity. Qed.
 
-  Example example_sql04_rhs_test01
-    : (Hs.parseSQL ∘ Hs.printSQL ∘ Hs.injection "z"%string "' or 1=1"%string $ sql04)
-    = Some (Hs.sqlSFW Hs.star "t" (Some (Hs.termPred (Hs.equalTerm (Hs.ColName "id") (Hs.IntVal 123)))), ""%string).
-  Proof. reflexivity. Qed.
+Definition sql02 : Hs.sql :=
+  Hs.sqlSFW (Hs.colNames ["c1"%string]) "t"%string None.
 
-  Example example_sql04_test01
-    : (spec sql04 "z"%string "' or 1=1"%string)
-    = true.
-  Proof. reflexivity. Qed.
+Example sql02_example1
+  (sql := sql02)
+  (x := "z"%string)
+  (v := "' or 1=1"%string)
+  : must_return_true sql x v
+  = true.
+Proof. reflexivity. Qed.
 
-  Definition sql07 : Hs.sql :=
-    Hs.sqlSFW Hs.star "t" (Some (Hs.termPred (Hs.equalTerm (Hs.ColName "name"%string) (Hs.Var "z"%string)))).
+Definition sql03 : Hs.sql :=
+  Hs.sqlSFW (Hs.colNames ["c1"%string; "c2"%string; "c3"%string]) "t"%string None.
 
-  Example example_sql07_rhs_test01
-    : (Hs.parseSQL ∘ Hs.printSQL ∘ Hs.injection "z"%string "' or 1=1"%string $ sql07)
-    = Some (Hs.sqlSFW Hs.star "t" (Some (Hs.termPred (Hs.equalTerm (Hs.ColName "name") (Hs.StrVal "' or 1=1")))), ""%string).
-  Proof. reflexivity. Qed.
+Example sql03_example1
+  (sql := sql03)
+  (x := "z"%string)
+  (v := "' or 1=1"%string)
+  : must_return_true sql x v
+  = true.
+Proof. reflexivity. Qed.
 
-  Example example_sql07_test01
-    : (spec sql07 "z"%string "' or 1=1"%string)
-    = true.
-  Proof. reflexivity. Qed.
+Definition sql04 : Hs.sql :=
+  Hs.sqlSFW Hs.star "t" (Some (Hs.termPred (Hs.equalTerm (Hs.ColName "id") (Hs.IntVal (123)%Z)))).
 
-  Definition sql10 : Hs.sql :=
-    Hs.sqlSFW Hs.star "t" (Some (Hs.orPred (Hs.termPred (Hs.equalTerm (Hs.ColName "name"%string) (Hs.StrVal "'abc'"))) (Hs.termPred (Hs.equalTerm (Hs.IntVal 1) (Hs.IntVal 1))))).
+Example sql04_example1
+  (sql := sql04)
+  (x := "z"%string)
+  (v := "' or 1=1"%string)
+  : must_return_true sql x v
+  = true.
+Proof. reflexivity. Qed.
 
-  Example example_sql10_rhs_test01
-    : (Hs.parseSQL ∘ Hs.printSQL ∘ Hs.injection "z"%string "' or 1=1"%string $ sql10)
-    = Some (Hs.sqlSFW Hs.star "t" (Some (Hs.orPred (Hs.termPred (Hs.equalTerm (Hs.ColName "name") (Hs.StrVal "'abc'"))) (Hs.termPred (Hs.equalTerm (Hs.IntVal 1) (Hs.IntVal 1))))), ""%string).
-  Proof. reflexivity. Qed.
+Definition sql05 : Hs.sql :=
+  Hs.sqlSFW Hs.star "t" (Some (Hs.termPred (Hs.equalTerm (Hs.ColName "id") (Hs.Var "z")))).
 
-  Example example_sql10_test01
-    : (spec sql10 "z"%string "' or 1=1"%string)
-    = true.
-  Proof. reflexivity. Qed.
+Example sql05_example1
+  (sql := sql05)
+  (x := "z"%string)
+  (v := "' or 1=1"%string)
+  : must_return_true sql x v
+  = true.
+Proof. reflexivity. Qed.
+
+Definition sql06 : Hs.sql :=
+  Hs.sqlSFW Hs.star "t" (Some (Hs.termPred (Hs.equalTerm (Hs.ColName "id") (Hs.StrVal "Hong")))).
+
+Example sql06_example1
+  (sql := sql06)
+  (x := "z"%string)
+  (v := "' or 1=1"%string)
+  : must_return_true sql x v
+  = true.
+Proof. reflexivity. Qed.
+
+Definition sql07 : Hs.sql :=
+  Hs.sqlSFW Hs.star "t" (Some (Hs.termPred (Hs.equalTerm (Hs.ColName "name"%string) (Hs.Var "z"%string)))).
+
+Example sql07_example1
+  (sql := sql07)
+  (x := "z"%string)
+  (v := "' or 1=1"%string)
+  : must_return_true sql x v
+  = true.
+Proof. reflexivity. Qed.
+
+Definition sql08 : Hs.sql :=
+  Hs.sqlSFW (Hs.colNames ["c1"%string]) "t" None.
+
+Example sql08_example1
+  (sql := sql08)
+  (x := "z"%string)
+  (v := "' or 1=1"%string)
+  : must_return_true sql x v
+  = true.
+Proof. reflexivity. Qed.
+
+Definition sql09 : Hs.sql :=
+  Hs.sqlSFW (Hs.colNames ["c1"%string; "c2"%string; "c3"%string]) "t" None.
+
+Example sql09_example1
+  (sql := sql09)
+  (x := "z"%string)
+  (v := "' or 1=1"%string)
+  : must_return_true sql x v
+  = true.
+Proof. reflexivity. Qed.
+
+Definition sql10 : Hs.sql :=
+  Hs.sqlSFW Hs.star "t" (Some (Hs.orPred (Hs.termPred (Hs.equalTerm (Hs.ColName "name") (Hs.StrVal "'abc'"))) (Hs.termPred (Hs.equalTerm (Hs.IntVal 1) (Hs.IntVal 1))))).
+
+Example sql10_example1
+  (sql := sql10)
+  (x := "z"%string)
+  (v := "' or 1=1"%string)
+  : must_return_true sql x v
+  = true.
+Proof. reflexivity. Qed.
+
+End SQL_EXAMPLES.
+
+Lemma String_values
+  : forall str, forall rest, Hs.sqlstringP (Hs.ppString str ++ rest)%string = Some (str, rest).
+Proof.
+Admitted.
+
+Theorem main_thm (s : Hs.sql) (x : string) (v : string)
+  : must_return_true s x v
+  = true.
+Proof.
+Admitted.
 
 End Main.
